{
 "cells": [
  {
   "cell_type": "markdown",
   "id": "a4ddca7b",
   "metadata": {},
   "source": [
    "note: the \"spectrum of A\" is defined on page 75 as $\\sigma(A)$ i.e. the complement of the set of regular points.  Many questions in this chapter ask the reader to \"find the spectrum\" of some operator though the official solutions give a refinement-- i.e. they show the details of $\\sigma(A)=\\sigma_p(A)\\cup\\sigma_c(A)\\cup\\sigma_r(A)$ [p. 76] which is interesting but more granular than what is actually asked--i.e. the exercises *don't* actually ask to find the spectrum and tripartition it into point, continuous and residual.  "
   ]
  },
  {
   "cell_type": "code",
   "execution_count": null,
   "id": "e8504c8f",
   "metadata": {},
   "outputs": [],
   "source": []
  },
  {
   "cell_type": "markdown",
   "id": "24f45111",
   "metadata": {},
   "source": [
    "**1.**   \n",
    "Find the spectrum of  the operator $D_w$ that operates on $\\mathscr l_2$ defined by \n",
    "\n",
    "$D_w x =\\begin{bmatrix}w_1\\cdot x_1 \\\\ w_2\\cdot x_2  \\\\ w_3\\cdot x_3\\\\\\vdots \\end{bmatrix}=w\\circ x$ \n",
    "\n",
    "remark: this should say a *bounded* operators as that is all we have a definition of spectrum for at this point; recall exercise 1 from the prior chapter that $\\Vert D_w\\Vert =\\sup_j\\vert w_j\\vert$   \n",
    "\n",
    "\n",
    "referring the definition of spectrum, we are looking for $\\lambda$ such that $\\big(D_w -\\lambda I\\big)$ is not bijective, and equivalently that bounded $ \\big(D_w -\\lambda I\\big)^{-1}$ doesn't exist  \n",
    "[recalling we work on Banach spaces only and Theorem 4.7.1 Banach Open Map Theorem for the boundedness of the inverse].  \n",
    "\n",
    "Now recall ex 4.8.1 and $\\big(D_w -\\lambda I\\big)$ is not invertible *iff* $\\inf_j \\vert w_j- \\lambda\\vert =0$  \n",
    "$\\implies \\sigma\\big(D_w\\big)= \\big\\{\\lambda \\in \\mathbb C: \\inf_j \\vert w_j- \\lambda\\vert =0\\big\\}$"
   ]
  },
  {
   "cell_type": "markdown",
   "id": "82a79d6c",
   "metadata": {},
   "source": [
    "**2.**  \n",
    "Find the spectrum of the operator $A$ in $L_2[-1,1]$ which is given by $(Af)(t)=a(t)\\cdot f(t)$ where   \n",
    "$a(t)=t$ for $t\\in[0,1]$ and $a(t)=0$ for $t\\in [-1,0]$  \n",
    "(errata: the text said $a(t)=0$ for $t\\in [-1,1)$ which is a contradiction)  \n",
    "\n",
    "\n",
    "If $\\lambda\\not\\in [0,1]$ then $\\lambda$ is regular since   \n",
    "$\\big(A-\\lambda I\\big):f\\mapsto (a-\\lambda)\\cdot f $ which has an inverse given by  \n",
    "$g\\mapsto (a-\\lambda)^{-1}\\cdot g $ since $a(t)-\\lambda$ is continuous and non-zero everywhere hence multiplying by $(a-\\lambda)^{-1}$ is a continuous mapping -- and it is bounded on $[-1,1]$ for reasons of compactness so $(a-\\lambda)^{-1}\\cdot g\\in L_2[-1,1]$ per Cauchy-Schwarz.  \n",
    "\n",
    "$\\sigma(A)=[0,1]$    \n",
    "Consider the constant map $f(t)=1$ and $\\lambda \\in [0,1]$    \n",
    "$\\implies \\big(A-\\lambda I\\big):f\\mapsto (a-\\lambda)\\cdot f $\n",
    "which is zero at $t=\\lambda$ so if $\\big(A-\\lambda I\\big)^{-1}$ existed then it would have the mapping  \n",
    "$g:\\mapsto (a-\\lambda)^{-1}\\cdot g $ almost everywhere and while we can duck the definition at $t=\\lambda$ specifically and e.g. assign it to be $1$ the issue is $\\big(A-\\lambda I\\big)^{-1}$ cannot be defined anywhere in a neighborhood containing $\\lambda$ since that set would have positive measure and the inverse mapping applies to constant $f$, above would have to be equal to $f\\mapsto (a-\\lambda)^{-1}\\cdot f=(a-\\lambda)^{-1} $ almost everywhere but that is not square integrable -- essentially for the same reason that $\\int_0^1\\frac{1}{x^2}=\\infty$ and in some ways echoes some of the examples in ex 2.4.27   \n",
    "\n",
    "note: the above argument seems to require some notions from measure theory which is a bit awkward since the authors insist measure theory is not needed until the 'second semester' [i.e. chapters $8+$]  "
   ]
  },
  {
   "cell_type": "markdown",
   "id": "a3dc92a4",
   "metadata": {},
   "source": [
    "**3.**  \n",
    "$A\\in L(X)$ be an invertible operator. Prove that $\\sigma\\left(A^{-1}\\right)=\\big\\{\\lambda^{-1}: \\lambda \\in \\sigma(A)\\big\\}$  \n",
    "\n",
    "For invertible [bounded] operator $T$ we argue, for $\\lambda \\neq 0$  \n",
    "$\\lambda \\text{ is a regular point of }T\\implies \\lambda^{-1} \\text{ is a regular point of }T^{-1}$  \n",
    "$\\big(T-\\lambda I\\big)=T\\big(I-\\lambda T^{-1}\\big)=-\\lambda \\cdot T\\big(-\\lambda^{-1}I + T^{-1}\\big)=-\\lambda \\cdot T\\big( T^{-1}-\\lambda^{-1}I\\big)$  \n",
    "where the RHS is invertible since the LHS is, and in particular $\\big( T^{-1}-\\lambda^{-1}I\\big)$ is invertible so $\\lambda^{-1}$ is regular for $T^{-1}$.  Of course trivially $0$ is regular for $T$ and $T^{-1}$ since it is invertible.  \n",
    "\n",
    "Letting $T:=A$ then the above yields for $\\lambda\\neq 0$   \n",
    "$\\lambda \\text{ is a regular point of }A\\implies \\lambda^{-1} \\text{ is a regular point of }A^{-1}$  \n",
    "\n",
    "and letting $T:=A^{-1}$ then the above yields for $\\lambda\\neq 0$    \n",
    "$\\lambda \\text{ is a regular point of }A^{-1}\\implies \\lambda^{-1} \\text{ is a regular point of }A\\iff \\lambda^{-1} \\text{ is a regular point of }A^{-1}\\implies \\lambda \\text{ is a regular point of }A$  \n",
    "where we use the automorphism of $z\\mapsto z^{-1}$ on the punctured plane $\\mathbb C\\sim\\big\\{0\\big\\}$ to get the \"$\\iff$\" equivalence    \n",
    "\n",
    "conclude for $\\lambda\\neq 0$  \n",
    "$\\lambda\\text{ is a regular point of }A\\iff \\lambda^{-1} \\text{ is a regular point of }A^{-1}$  \n",
    "and again trivially $A$ and $A^{-1}$ have zero as a regular point.  \n",
    "\n",
    "Looking at set complements then, $\\lambda \\in \\sigma\\big(A\\big)\\iff \\lambda^{-1}\\in \\sigma\\big(A^{-1}\\big)$  \n"
   ]
  },
  {
   "cell_type": "markdown",
   "id": "35a35ae4",
   "metadata": {},
   "source": [
    "**4.**  \n",
    "$A\\in L(X)$ and $\\lambda \\in \\mathbb C$ an assume that there exists a sequence $(x_n)_{n=1}^\\infty \\subseteq X$ such that $\\Vert x_n\\Vert =1$ and $Ax_n-\\lambda x_n\\to 0$ as $n\\to \\infty$.  Prove  that $\\lambda \\in \\sigma(A)$.  \n",
    "\n",
    "*suppose for contradiction* that $\\lambda$ is a regular point, i.e. that $\\big(A-\\lambda\\big)^{-1}$ exists  \n",
    "[recalling we work solely on Banach spaces so per Theorem 4.7.1, Banach Open Map Theorem, a bounded linear map is bijective *iff* it has a bounded inverse]  \n",
    "\n",
    "then with $\\big(A-\\lambda I\\big)x_n:=y_n$ we have for all $n$  \n",
    "$\\big\\Vert \\big(A-\\lambda I\\big)^{-1}y_n\\big\\Vert  = \\big\\Vert \\big(A- I \\lambda\\big)^{-1}\\big(A-\\lambda I\\big)x_n\\big\\Vert = \\big\\Vert x_n\\big\\Vert =1$  \n",
    "but for any $\\epsilon \\gt 0$ we know $\\Vert y_n\\Vert \\lt \\epsilon$ for all $n\\geq N$ (large enough)  \n",
    "\n",
    "hence for $n\\geq N$  \n",
    "$\\implies \\big\\Vert \\big(A-\\lambda I\\big)^{-1}\\frac{y_n}{\\Vert y_n\\Vert}\\big\\Vert = \\frac{1}{\\Vert y_n\\Vert}\\gt \\frac{1}{\\epsilon}\\implies \\big\\Vert \\big(A-\\lambda I \\big)^{-1}\\big\\Vert \\gt \\frac{1}{\\epsilon}$ \n",
    "$\\implies \\big(A-\\lambda I\\big)^{-1}$ is unbounded, since $\\epsilon \\gt 0$ was arbitrary, a contradiction  \n"
   ]
  },
  {
   "cell_type": "markdown",
   "id": "0d35ca45",
   "metadata": {},
   "source": [
    "**extension:**  \n",
    "we can slightly modify the above to make a (partial) converse to ex 4.8.24 [which roughly mimics exercise 3.27 in MacCluer]  \n",
    "\n",
    "suppose $A\\in B(H_1, H_2)$ and the image of $A$ is closed. Then for $v \\in (\\ker A)^\\perp$ we have  \n",
    "$\\big\\Vert Av \\big\\Vert\\geq m\\cdot \\big\\Vert v\\big\\Vert$ for some $m\\gt 0$.  \n",
    "\n",
    "\n",
    "First notice that $\\text{image }A=\\overline{\\text{image }A}\\subseteq H_2$ implies that $\\text{image }A$ is a complete subspace of $H_2$ hence it is a Banach space in its own right.  Similarly $(\\ker A)^\\perp\\subseteq H_1$ is always a closed subspace hence Banach.  \n",
    "This means we can define a map $T:(\\ker A)^\\perp\\rightarrow \\text{image }A$ given by $v\\mapsto Av$ which is by construction injective and surjective so a formal linear inverse $T^{-1}$ exists. And $T^{-1}\\in B(H_2, H_1)$ by Banach Open Mapping theorem. Thus setting $m:=\\frac{1}{\\Vert T^{-1} \\Vert}$ proves the claim.  Put differently, mimicking the above argument, if the claim is not true we have some sequence $v_k$ with $\\Vert v_k\\Vert =1$ such that $Tv_k\\to 0\\implies \\Vert v_k\\Vert = \\Vert T^{-1}Tv_k\\Vert= \\Vert T^{-1}y_k\\Vert =1$  which implies $T^{-1}$ is unbounded, contradicting the Banach Open Mapping theorem.  \n"
   ]
  },
  {
   "cell_type": "markdown",
   "id": "d6084701",
   "metadata": {},
   "source": [
    "**5.**  \n",
    "Let $\\mathbb C_{\\mathbb R}$ be the space of all continuous and bounded functions $x(t)$ on $\\mathbb R$ with norm $\\Vert x\\Vert =\\sup_{t\\in \\mathbb R}\\vert x(t)\\vert$.  On the space $C_{\\mathbb R}$ we define the operator $A$ by $(Ax)(t) = x(t+s)$ where $s\\in \\mathbb R$ is a constant.  Prove $\\sigma(A) =\\big\\{\\lambda \\in \\mathbb C:\\vert \\lambda \\vert =1\\big\\}$  \n",
    "\n",
    "*remark:* evidently $x:\\mathbb R\\longrightarrow \\mathbb C$  \n",
    "\n",
    "Note by inspection $\\big\\Vert A x\\big\\Vert=\\big\\Vert  x\\big\\Vert$ so $A$ is unitary where $\\Vert A \\Vert =1$ and that $A^{-1}$ exists and is given by $(Ax)(t) = x(t-s)$  which is unitary with norm 1 as well.  \n",
    "\n",
    "$\\sigma(A) \\subseteq\\big\\{\\lambda \\in \\mathbb C:\\vert \\lambda \\vert =1\\big\\}$   \n",
    "per Prop 5.0.1 if $\\vert \\lambda \\vert \\gt 1 =\\Vert A\\Vert$ then $\\lambda \\not\\in\\sigma(A)$, i.e. a regular point.  \n",
    "and for $A^{-1}$ then $\\vert \\lambda\\vert \\lt 1\\implies \\vert \\lambda\\vert^{-1}\\gt \\left \\Vert A^{-1}\\right\\Vert =1 \\implies \\lambda^{-1} \\not\\in \\sigma\\left(A^{-1}\\right)$ per Prop 5.0.1 $\\implies \\lambda \\not\\in\\sigma(A)$ per exercise 3.  \n",
    "\n",
    "Now consider arbitrary $\\lambda$ where $\\vert \\lambda\\vert =1$, i.e. $\\lambda =\\exp\\big(2\\pi\\cdot i\\cdot \\theta\\big)$ for some $\\theta \\in \\big(0,2\\pi\\big]$.  We argue $\\big(A-\\lambda I\\big)$ has a non-trivial kernel [i.e. $\\lambda$ is point spectrum]. Being linear $\\big(A-\\lambda I\\big)\\mathbf 0=\\mathbf 0$, but consider $x_0(t):= \\exp\\big(2\\pi\\cdot i\\cdot \\frac{t}{r}\\big)$ where $r:= \\frac{s}{\\theta}$.  This map sends the real line to the unit circle.     \n",
    "$(Ax_0)(t)= \\exp\\big(2\\pi\\cdot i\\cdot \\frac{t+s}{r}\\big)= \\exp\\big(2\\pi\\cdot i\\cdot \\frac{t+s}{r}\\big)=\\exp\\big(2\\pi\\cdot i\\cdot \\frac{t}{r}\\big)\\cdot \\exp\\big(2\\pi\\cdot i\\cdot \\frac{s}{r}\\big)=x_0(t)\\cdot \\exp\\big(2\\pi\\cdot i\\cdot \\frac{s}{r}\\big)=\\lambda \\cdot x_0(t) $  \n",
    "$\\implies \\big(A-\\lambda I\\big)x_0= \\lambda \\cdot x_0 -\\lambda \\cdot x_0=0$  "
   ]
  },
  {
   "cell_type": "markdown",
   "id": "bf73cc28",
   "metadata": {},
   "source": [
    "**8.**  \n",
    "Let $A$ be an invertible operator and let $K$ be a compact operator in a Banach space, $X$.  Prove that \n",
    "\n",
    "(a.) $\\dim \\ker\\big(A+K\\big)\\lt \\infty$  \n",
    "re-write this as  \n",
    "$\\dim \\ker\\big(A+K\\big)=\\dim \\ker\\big(A(I+A^{-1}K)\\big)=\\dim \\ker\\big(I+A^{-1}K\\big)\\lt \\infty$  \n",
    "Working from right to left:  \n",
    "where the RHS holds by Prop 5.2.4, with $\\lambda :=-1$ and  the 2nd to right equality holds because invertible linear maps preserve finite dimensions.  Also recall $A^{-1}K$, as well as  $KA^{-1}$, is compact per Prop 4.3.4  \n",
    "\n",
    "(b.) $\\text{codim } \\text{Image}\\big(A+K\\big)\\lt \\infty$  \n",
    "re-write this as  \n",
    "$\\text{codim } \\text{Image}\\big(A+K\\big)=\\text{codim } \\text{Image}\\big(A(I+A^{-1}K)\\big)=\\text{codim } \\text{Image}\\big(A(A^{-1}K+I)\\big)\\lt\\infty$   \n",
    "*remark: the below argument actually yields an independent proof of exercise 5.3.13 Fredholm's third theorem*  \n",
    "\n",
    "We prove this as follows.  Let $T$ be compact with $\\dim \\ker \\big(T + I\\big)=m\\lt \\infty$ [here $\\lambda:=-1$ with Prop 5.2.4 applied].  Letting $L:=\\text{Image }\\big(T + I\\big)$ we have $L$ is closed per Prop 5.2.5 \n",
    "\n",
    "Base Case: $m=1$    \n",
    "Since $\\dim \\ker \\big(T + I\\big)=1$ we have $\\ker \\big(T+I\\big)=\\text{span}\\big\\{w\\big\\}$ and  some $y \\not\\in L$ per Prop 5.2.7.  Per [Hahn-Banach] Corollary 3.1.7 there is an $f \\in X^*$ such with norm $1$ such that $f(w) \\gt 0$.  \n",
    "\n",
    "$B:= \\big(T+I\\big) +f(x)\\cdot y$ noting that $Bw= f(w)\\cdot y\\neq 0\\implies y \\in \\text{image }\\big(B\\big)$  \n",
    "$v \\in \\ker B\\implies -\\big(T+I\\big)v = f(v)\\cdot y$  \n",
    "$\\implies -\\big(T+I\\big)v \\in L \\cap \\text{span}\\big\\{y\\big\\}\\implies -\\big(T+I\\big)v = 0= f(v)\\cdot y$  $\\implies v \\in \\ker \\big(T+I\\big)\\implies v =\\alpha \\cdot w\\implies 0=f(v)\\cdot y=0=f(\\alpha\\cdot w)\\cdot y=\\alpha\\cdot f( w)\\cdot y\\implies \\alpha =0 \\implies v=0$  \n",
    "$\\implies \\dim \\ker B =0\\implies \\text{image }B=X \\quad\\text{(prop 5.2.10)}$  \n",
    "\n",
    "$\\implies X = \\text{image }\\big(T+I\\big)\\oplus\\text{span}\\big\\{y\\big\\}$  \n",
    "$\\implies X \\big/\\big(T+I\\big)\\cong \\text{span}\\big\\{y\\big\\}$  \n",
    "i.e. this sets the stage for an induction that $\\dim \\big/\\big(T+I\\big) = \\dim \\ker \\big(T+I\\big)$  \n",
    "\n",
    "Inductive Case: $m\\geq 2$  \n",
    "The argument runs almost the same as in the Base Case, again reducing the the dimension of the kernel by one and finishing with induction hypothesis.  \n",
    "Since $\\dim \\ker \\big(T + I\\big)=m$ we have $\\ker \\big(T+I\\big)=\\text{span}\\big\\{w_1, \\dotso, w_{m-1}, w_m\\big\\}$ and some $y_m \\not\\in L$ per Prop 5.2.7.  Per [Hahn-Banach] Corollary 3.1.7 there is an $f \\in X^*$ such with norm $1$ such that $f(w_m) \\gt 0$ and $f\\big(\\text{span}\\big\\{w_1, \\dotso, w_{m-1}\\big\\}\\big)=\\big\\{0\\big\\}$ since $\\text{span}\\big\\{w_1, \\dotso, w_{m-1}\\big\\}$ is closed [ex 3.3.3].  \n",
    "\n",
    "$B:= T+I +f(x)\\cdot y_m$  [where $T+  f(x)\\cdot y_m$ is the sum of two compact operators so compact per Prop 4.3.4]     \n",
    "$v \\in \\ker B\\implies -\\big(T+I\\big)v = f(v)\\cdot y_m$  \n",
    "$\\implies -\\big(T+I\\big)v \\in L \\cap \\text{span}\\big\\{y_m\\big\\}\\implies -\\big(T+I\\big)v = 0= f(v)\\cdot y_m$  $\\implies v \\in \\ker \\big(T+I\\big)\\implies v =\\sum_{k=1}^m \\lambda_k \\cdot w_k\\implies 0=f\\big(\\sum_{k=1}^m \\lambda_k \\cdot w_k\\big)\\cdot y_m = \\sum_{k=1}^m \\lambda_k \\cdot f\\big( w_k\\big)\\cdot y_m = \\lambda_m \\cdot f\\big(w_m\\big)\\cdot y_m $  \n",
    "$\\implies \\lambda_m =0 \\implies v \\in \\text{span}\\big\\{w_1, \\dotso, w_{m-1}\\big\\}$  \n",
    "$\\implies \\dim \\ker B \\leq m-1 \\implies \\dim \\ker B = m-1 \\quad\\text{(check by setting }v:=w_j\\text{ for }1\\leq j\\leq m-1\\text{)}$  \n",
    "\n",
    "and by calling on induction hypothesis we get  \n",
    "$\\implies X = \\text{image }\\big(B\\big)\\oplus \\text{span}\\big\\{y_1, \\dotso, y_{m-1}\\big\\}=\\text{image }\\big(T+I\\big)\\oplus \\text{span}\\big\\{y_m\\big\\}\\oplus \\text{span}\\big\\{y_1, \\dotso, y_{m-1}\\big\\}$  \n",
    "where the 2nd equality comes from checking  $B(w_m) =f(w_m)\\cdot y_m\\neq 0$ and for any $v \\in \\text{image}(T+I)$ we have $(T+I)x =v$ for some $x$ which implies $B(x+\\alpha \\cdot w_m)=v$ for suitable choice of $\\alpha$ so $\\text{image }B \\supseteq \\text{image}(T+I)\\oplus \\text{span}\\big\\{y_m\\big\\}$  . Conversely if $v\\in \\text{image }B$ then $Bx=v =(T+I)x +f(x)\\cdot y_m\\implies \\text{image }B \\subseteq \\text{image}(T+I)\\oplus \\text{span}\\big\\{y_m\\big\\}$   \n",
    "$\\implies X =\\text{image }\\big(T+I\\big)\\oplus \\text{span}\\big\\{y_1, \\dotso, y_{m-1},y_m\\big\\}$  \n",
    "$\\implies X \\big/\\text{image}\\big(T+I\\big)\\cong \\text{span}\\big\\{y_1, \\dotso, y_{m-1},y_m\\big\\}$  \n",
    "$\\implies X \\big/\\text{image}\\big(T+I\\big) = \\dim \\text{span}\\big\\{y_1, \\dotso, y_{m-1},y_m\\big\\} = m =\\dim \\ker \\big(T+I\\big)$  \n",
    "\n",
    "Finally, let $A^{-1}K:= T$  \n",
    "$\\implies X =\\text{image }\\big(A^{-1}K+I\\big)\\oplus \\text{span}\\big\\{y_1, \\dotso, y_{m-1},y_m\\big\\}$  \n",
    "$\\implies AX =X =\\text{image }\\Big(A\\big(A^{-1}K+I\\big)\\Big)\\oplus \\text{span}\\big\\{Ay_1, \\dotso, Ay_{m-1},Ay_m\\big\\}=\\text{image }\\Big(A\\big(A^{-1}K+I\\big)\\Big)\\oplus \\text{span}\\big\\{z_1, \\dotso, z_{m-1},z_m\\big\\}$  \n",
    "$\\implies X \\big/\\text{image }\\Big(A\\big(A^{-1}K+I\\big)\\Big)\\cong \\text{span}\\big\\{z_1, \\dotso, z_{m-1},z_m\\big\\}$  \n",
    "which has dimension $m\\lt \\infty$ as required by the problem.  \n",
    "\n",
    "*remark:*  \n",
    "The technique here is very much that same as what we'd do in linear algebra.  E.g. the approach for $A \\in \\mathbb F^{n\\times n}$: if $0\\neq v \\in \\ker A$, we can reduce the kernel size of $A$ by one [and of course increase its rank by one] as follows: construct invertible matrix $V$ with its first column being $v$ and any other (chosen) basis vectors for $\\ker A$ being columns $v_k$ for $2\\leq k\\leq \\dim \\ker A=r$ of $V$ then append standard basis vectors as relevant for other columns to get an invertible matrix.  Let $W:=V^{-1}=\\begin{bmatrix}\\mathbf w_1^T   \\\\\\vdots \\\\ \\mathbf w_n^T\\end{bmatrix}$ and $\\implies \\dim \\ker \\big(A+\\mathbf v\\mathbf w_1^T\\big)=1+\\dim \\ker A $  \n",
    "\n",
    "which we can check since  \n",
    "$\\big(A+\\mathbf v\\mathbf w_1^T\\big)V = AV + \\mathbf v\\mathbf w_1^TV = V \\begin{bmatrix} \\mathbf 0 &*\\\\ \\mathbf 0 & A_{n-r}\\end{bmatrix}+V \\begin{bmatrix} D_r &\\mathbf 0\\\\ \\mathbf 0 & \\mathbf 0\\end{bmatrix}= V \\begin{bmatrix} D_r &*\\\\ \\mathbf 0 & A_{n-r}\\end{bmatrix}$  \n",
    "where $D_r$ is diagonal with the top left entry $=1$ and all else equal to zero and $\\det\\big(A_{n-r}\\big)\\neq 0$.  By sub-additivity of rank we have $\\text{rank}\\big(A+\\mathbf v\\mathbf w_1^T\\big)\\leq \\text{rank}A +1$ and this is met with equality since the bottom $n-r$ rows are linearly independent (since $A_{n-r}$ is invertible) and the top row is linearly independent of those by inspection [alternatively consider the $n-r+1\\times n-r+1$ principal submatrix containing $A_{n-r}$ and the top left entry of $D_r$ which has determinant $=1\\cdot \\det\\big(A_{n-r}\\big)\\neq 0$]  \n",
    "\n",
    "**deriving Fredholm's Third Theorem**  \n",
    "the above argument implies Fredholm's Third Theorem as follows.  First note that for compact $T'$ and $\\lambda \\neq 0$ we may re-write $\\text{image}\\big(T'-\\lambda I\\big)=\\text{image}\\big(-\\lambda \\cdot\\big(\\frac{T'}{-\\lambda}+I \\big)\\Big)=\\text{image}\\big(\\frac{T'}{-\\lambda}+I \\big)=\\text{image}\\big(T+I \\big)$ \n",
    "\n",
    "so it suffices to consider $\\big(T+I\\big)$ as was done above [i.e. WLOG $\\lambda =-1$].  Now referring to page 81, consider solutions to  \n",
    "$Tx - \\lambda \\cdot x = v = (T+I)x $  \n",
    "$\\implies v \\in \\text{image}\\big(T+I\\big)\\iff f_i(v)=0\\text{ for all }i\\in\\big\\{1,\\dotso, k\\big\\}$ \n",
    "where $\\big\\{f_1,\\dotso, f_k\\big\\}$ forms a basis for $\\ker (T^*)_\\overline{\\lambda}=\\ker T^*_{-1}$ [i.e. annihilators of the image of $T+I$ in line with Prop 5.2.8(i)]   \n",
    "\n",
    "Applying ex 3.3.9 we can derive [necessarily linearly independent] $\\big\\{x_1, \\dotso, x_k\\big\\}\\in X$ such that  \n",
    "$f_i(x_j)= \\delta_{i,j}$  \n",
    "$\\implies \\text{span}\\big\\{x_1, \\dotso, x_k\\big\\}\\cap \\text{image }\\big(T+I\\big)=\\big\\{0\\big\\}$ by checking the subspaces under the image of  $f\\in\\big\\{f_1,\\dotso, f_k\\big\\}$  \n",
    "$\\implies \\text{image }\\big(T+I\\big)\\oplus \\text{span}\\big\\{x_1, \\dotso, x_k\\big\\}\\subseteq X =\\text{image }\\big(T+I\\big)\\oplus \\text{span}\\big\\{y_1, \\dotso, y_{m-1},y_m\\big\\}$   \n",
    "$\\implies k\\leq m$  \n",
    "by quotienting each side by $\\text{image }\\big(T+I\\big)$.  \n",
    "\n",
    "\n",
    "Re-using the Gram type matrix in ex 3.3.9 we get  \n",
    "$G=\\begin{bmatrix}\n",
    "    f_1(y_1) & \\dots& f_{k-1}(y_1) &f_{k}(y_1) \\\\\n",
    "    f_1(y_2) &   \\dots & f_{k-1}(y_2)& f_k(y_2)\\\\\n",
    "    \\vdots & \\ddots & \\ddots & \\vdots\\\\\n",
    "    f_1(y_{m-1}) & \\dots & f_{k-1}(y_{m-1})& f_k(y_{m-1})\\\\\n",
    "    f_1(y_{m}) & \\dots & f_{k-1}(y_{m}) & f_k(y_{m}) \\\\\n",
    "    \\end{bmatrix}$  \n",
    "where $G\\in \\mathbb C^{m\\times k}$. Now consider the left nullspace, i.e. any $\\mathbf a$ such that \n",
    "$\\mathbf a^TG =\\mathbf 0^T\\implies f_i\\big(v\\big)=0 \\text{ for }1\\leq i\\leq m$  with $v:= \\sum_{j=1}^m a_j \\cdot y_j$  \n",
    "$\\implies v \\in \\text{image }\\big(T+I\\big)$  by commentary at bottom of page 81 [i.e. since the $f_i$ don't kill it, $(T+I)x=v$ is valid]   \n",
    "$\\implies v \\in \\text{image }\\big(T+I\\big)\\cap \\text{span}\\big\\{y_1, \\dotso, y_{m-1},y_m\\big\\}\\implies v =0$  \n",
    "since $X=\\text{image }\\big(T+I\\big)\\oplus \\text{span}\\big\\{y_1, \\dotso, y_{m-1},y_m\\big\\}$  \n",
    "$\\implies \\mathbf a =\\mathbf 0\\text{ since }0=v= \\sum_{j=1}^m a_j \\cdot y_j$ and  the $y_j$ are linearly independent  \n",
    "$\\implies \\dim \\ker G^T=0\\implies m\\leq k\\quad \\text{(e.g. by rank-nullity for  }G^T\\text{)}$  \n",
    "\n",
    "conclude: $\\dim \\ker \\big(T+I\\big)= m =k =\\ker \\big(T+I\\big)^* $\n",
    "\n",
    "*remark:*  \n",
    "a different way to argue $m=k$ would be to observe  \n",
    "$v \\not\\in \\text{image}\\big(T+I\\big)\\iff  [v]\\neq [0] \\in X\\big/\\text{image}\\big(T+I\\big) \\iff f_i(v)\\neq 0\\text{ for some }i\\in\\big\\{1,\\dotso, k\\big\\}$ so define $E_i:= \\ker f_i$   \n",
    "Now consider $0\\neq v \\in \\text{span}\\big\\{y_1,\\dotso, y_m\\big\\}\\implies [0]\\neq [v]\\in X\\big / \\big(\\bigcap_{i=1}^k E_i\\big)$ i.e. the quotient maintains linear independence of $y_m$ but we know   \n",
    "$\\dim X\\big / \\big(\\bigcap_{i=1}^k E_i\\big)\\leq k$ per ex 1.6.3 $\\implies m\\leq k$. Using $\\big\\{x_1, \\dotso, x_k\\big\\}$ one should be able to argue that in fact $\\dim X\\big / \\big(\\bigcap_{i=1}^k E_i\\big)= k$  and then that  $X\\big / \\big(\\bigcap_{i=1}^k E_i\\big) \\cong X\\big/\\text{image}\\big(T+I\\big)$ yielding $m=k$.  \n"
   ]
  },
  {
   "cell_type": "markdown",
   "id": "7d1d52cb",
   "metadata": {},
   "source": [
    "**11.**  \n",
    "Let $S_R$ and $S_L$ be the right and left shift operators respectively on $\\mathscr l_2$  i.e.  \n",
    "$S_R\\left( \\begin{bmatrix}x_1 \\\\ x_2  \\\\ x_3\\\\\\vdots \\end{bmatrix}\\right)=\\begin{bmatrix}0\\\\x_1 \\\\ x_2  \\\\\\vdots \\end{bmatrix}$\n",
    "\n",
    "$S_L\\left(\\begin{bmatrix}x_1 \\\\ x_2  \\\\ x_3\\\\\\vdots \\end{bmatrix}\\right)=\\begin{bmatrix}x_2  \\\\ x_3\\\\ x_4\\\\\\vdots \\end{bmatrix}$  \n",
    "\n",
    "Find the spectrum of these operators  \n",
    "\n",
    "Note that trivially $0\\in\\sigma(S_R)$ and $0\\in\\sigma(S_L)$ since $\\mathbf e_1 \\not\\in \\text{image }S_R$ and $\\mathbf e_1 \\in \\ker S_L$.  $S_R$ is unitary, but not surjective, so $\\Vert S_R\\Vert =1$\n",
    " and also $\\Vert S_L\\Vert =1$ though it is not unitary [check e.g. that it is contracting but preserves the norm of $\\mathbf e_2$] hence per Prop 5.0.1 any $\\vert \\lambda \\vert \\gt 1$ is a *regular point*.  Now consider any $\\lambda \\in B^*\\big(0,1\\big)\\cup \\partial B\\big(0,1\\big)=\\overline B\\big(0,1\\big)\\sim\\big\\{0\\big\\}$ i.e. the punctured closed unit ball.  \n",
    " \n",
    "\n",
    "\n",
    "\n",
    "$C_\\lambda := S_R -\\lambda I = \\lambda \\cdot \n",
    "\\left[\\begin{matrix}1 & 0 & 0 & 0 & 0&   \\dots \\\\\n",
    "-\\lambda^{-1} & 1 & 0 & 0 & 0 &  \\dots\\\\ \n",
    "0 & -\\lambda^{-1} & 1 & 0 & 0 &  \\dots\\\\\n",
    "0 & 0 & -\\lambda^{-1} & 1 & 0 &  \\dots\\\\\n",
    "\\vdots & \\vdots & \\vdots & \\ddots & \\ddots & \\ddots\\\\\n",
    "\\end{matrix}\\right]$  \n",
    "\n",
    "suppose $\\mathbf e_1 \\in \\text{image }C_\\lambda\\iff \\mathbf e_1=C_\\lambda x$ for some $x$   \n",
    "$\\implies x =\\begin{bmatrix}\\lambda^{-1} \\\\ \\lambda^{-2} \\\\ \\lambda^{-3}\\\\ \\lambda^{-4}\\\\\\vdots \\end{bmatrix}$  \n",
    "$\\implies \\big\\Vert x \\big \\Vert=\\infty$ which is a contradiction since $x \\in \\mathscr l_2$  \n",
    "conclude $C_\\lambda$ is not surjective (hence not invertible) so $\\lambda \\in \\sigma(S_R)$  \n",
    "\n",
    "For the Left shift operator  \n",
    "$B_\\lambda := S_L -\\lambda I = \\lambda \\cdot \n",
    "\\left[\\begin{matrix}1 & -\\lambda^{-1} & 0 & 0 & 0&   \\dots \\\\\n",
    "0 & 1 &- \\lambda^{-1} & 0 & 0 &  \\dots\\\\ \n",
    "0 & 0 & 1 & -\\lambda^{-1} & 0 &  \\dots\\\\\n",
    "0 & 0 & 0 & 1 &- \\lambda^{-1} &  \\dots\\\\\n",
    "\\vdots & \\vdots & \\vdots & \\ddots & \\ddots & \\ddots\\\\\n",
    "\\end{matrix}\\right]=C_\\lambda^T$  \n",
    "\n",
    "we'll solve for the first 3 standard basis vectors to uncover a pattern  \n",
    "$B_\\lambda x_1=\\mathbf e_1\\implies x_1 =\\begin{bmatrix}\\lambda^{-1} \\\\ 0 \\\\ 0\\\\ 0\\\\\\vdots \\end{bmatrix}$  \n",
    "\n",
    "$B_\\lambda x=\\mathbf e_2\\implies x_2 =\\begin{bmatrix}\\lambda^{-2} \\\\ \\lambda^{-1} \\\\ 0\\\\ 0\\\\\\vdots \\end{bmatrix}$  \n",
    "\n",
    "$B_\\lambda x=\\mathbf e_3\\implies x_3 =\\begin{bmatrix}\\lambda^{-3} \\\\ \\lambda^{-2} \\\\ \\lambda^{-1}\\\\ 0\\\\\\vdots \\end{bmatrix}$  \n",
    "and in general  \n",
    "$B_\\lambda x_n=\\mathbf e_n\\implies x_n=\\begin{bmatrix}\\lambda^{-n} \\\\ \\vdots \\\\ \\lambda^{-1}\\\\ 0\\\\\\vdots \\end{bmatrix}$ where formally induction is used to prove this final claim  \n",
    "\n",
    "Notice that while each $\\mathbf e_n$ has a solution, the $x_n$ end up with arbitrarily large lengths.  \n",
    "\n",
    "Then consider the sequence $\\big\\{\\frac{x_n}{\\Vert x_n\\Vert}\\big\\}$ in the unit sphere where $B_\\lambda \\frac{x_n}{\\Vert x_n\\Vert}= \\frac{\\mathbf e_n}{\\Vert x_n\\Vert}\\to \\mathbf 0 $  \n",
    "per exercise $4$ we know $B$ is not invertible hence $\\lambda \\in \\sigma(S_L)$.  As an aside, since each standard basis vector is in the image of $B_\\lambda$ this means $\\text{image }B_\\lambda$ is dense in $\\mathscr l_2$ so the spectrum here is either point spectrum or continuous spectrum.  \n",
    "\n",
    "- - - - -  \n",
    "\n",
    "note: page 77 indicates $S_R$ has spectrum being the open unit disc not closed unit disc... probably errata   "
   ]
  },
  {
   "cell_type": "markdown",
   "id": "8736b216",
   "metadata": {},
   "source": [
    "**12.**  \n",
    "\n",
    "Define the operator $K:L_2[0,1]\\rightarrow L_2[0,1]$ by  \n",
    "$$(Kf)(t)=\\int_0^1 k(t,s)\\cdot f(s)ds$$  \n",
    "\n",
    "where $k(t,s)=1$ for $0\\leq s\\leq t$ and $0$ otherwise.  Find the spectrum of $K$  \n",
    "\n",
    "*remark:*  I was not able to solve this problem as dealing with non-continuous and especially non-Riemann integrable $f$ is rather tricky here.  This appears to be an error and a more fitting problem statement would be $K:C[0,1]\\longrightarrow C[0,1]$.\n",
    "\n",
    "I step through the official solution with additional commentary, below.  Assume $\\lambda \\neq 0$  \n",
    "\n",
    "$K$ is compact per some mixture of ex 4.8.20 and/or page 61.  And via compactness we know $0\\in \\sigma(K)$ and any other spectrum is point spectrum [ref 5.2.3].  So consider  \n",
    "$$\\lambda \\cdot f(t)=(Kf)(t)=\\int_0^1 k(t,s)\\cdot f(s)ds$=\\int_0^t f(s)ds  $$  \n",
    "The solution then asserts \"hence it follows that $f$ is continuously differentiable\" presumably leaning on the Fundamental Theorem of Calculus which does not apply for non Riemann Integrable functions.  However if we think this through iteratively, *and use an intro to measure theory course*,  we can deduce that such an $f$ must be absolutely continuous hence continuous hence the FTC *does apply* and  \n",
    "$\\lambda \\cdot f(t)= F(t)-F(0)$  \n",
    "- - - -  \n",
    "But how one is supposed to deduce this without knowing measure theory is beyond me.  Recall that chapter 5 is in semester 1 for the book which *does not use measure theory* and for purposes of this semester we use the opaque definition that the above Lebesgue integral is the completion of the Riemann Integral.  The authors provide no justification for their assertion -- some kind of density argument would seemed necessary.   \n",
    "- - - -  \n",
    "returning to $\\lambda \\cdot f(t)= F(t)-F(0)$  and considering $t:=0\\implies f(0)=0$ and differentiating $\\lambda \\cdot f(t)= F(t)-F(0)\\implies \\lambda \\cdot f'(t)=f(t)$ which is known to have an exponential type solution, though awkwardly the authors don't justify this and this too is not part of the pre-reqs for semester one which are supposedly \"minimal amounts of linear algebra and calculus\".  However we can recall section 7 of chapter 4 in Artin's *Algebra* (1st ediition) to determine that \n",
    "$\\lambda \\cdot f'(t)=f(t)\\implies f(t)=c\\cdot \\exp\\big(\\lambda\\cdot t\\big)$ and $f(0)=0\\implies c=0\\implies f=0$ thus $f$ isn't an eigenvector and $\\lambda$ is not point-spectrum.  Conclude $\\sigma\\big(K\\big)=\\big\\{0\\big\\}$.  "
   ]
  },
  {
   "cell_type": "code",
   "execution_count": null,
   "id": "9978a250",
   "metadata": {},
   "outputs": [],
   "source": []
  },
  {
   "cell_type": "markdown",
   "id": "45e73c86",
   "metadata": {},
   "source": [
    "**13.**  \n",
    "Fredholm's third theorem:  \n",
    "Let $T$ be a compact operator in a Banach space.  Prove that $\\dim \\ker T_\\lambda=\\dim\\ker (T^*)_\\lambda$.  \n",
    "\n",
    "Hint: Set $\\dim \\ker T_{\\lambda} = n$ and $\\dim\\ker (T^*)_{\\overline{\\lambda}}=p$ and the select basis $\\big\\{x_1,\\dots, x_n\\big\\}$ for $\\ker T_\\lambda$  and let $\\big\\{f_1,\\dots, f_p\\big\\}$ be a basis for $\\ker (T^*)_{\\overline{\\lambda}}$.  Then take the functionals $\\phi_1, \\dotso, \\phi_n\\in X^*$ such that $\\phi_i(x_j)=\\delta_{ij}$ [Corollary 3.1.10] and the elements $u_1,\\dotso, u_p\\in X$ such that $f_i(u_j)=\\delta_{ij}$.  Assuming $n\\lt p$ consider the operator $Bx= Tx +\\sum_{k=1}^n \\phi_k(x)\\cdot u_k$ and show that $\\dim\\ker B_\\lambda =0$ but $\\dim \\ker (B^*)_{\\overline {\\lambda}}=0$.  For the case $p\\lt n$ consider the operator $Gh = T^*h + \\sum_{k=1}^p h(u_k)\\cdot \\phi_k$  \n",
    "\n",
    "remark: this should say, assume $\\lambda \\neq 0$ [for finiteness of kernel dimension in line with Prop 5.2.4, etc.].  \n",
    "**Also** a different proof is given as part of the above answer to *exercise 8*.   \n",
    "- - - -   \n",
    "\n",
    "\n",
    "Note: the $u_i$ existing such that $f_i(u_j)=\\delta_{ij}$ exist per ex 3.3.9.  There is no requirement here that the $f_i$ or the $u_i$ have norm 1 hence no contradiction with ex 3.3.7.  Also note that $B$ and $G$ are both compact since they are the sum of compact operators, which form a [two sided] ideal per Prop 4.3.4 and recall that bounded finite rank operators are compact [ref page 66].  Also note that the inner product notation from page 66 is quite helpful in dealing with this problem \n",
    "\n",
    "**suppose for contradiction** that $n\\lt p$   \n",
    "$v \\in \\ker B_\\lambda \\implies -T_\\lambda v =\\sum_{k=1}^n \\phi_k(v)\\cdot u_k$  \n",
    "$\\implies 0 = \\big\\langle  v, 0\\big\\rangle= \\big\\langle  v, (T^*)_\\overline{\\lambda} f_i\\big\\rangle =-\\big\\langle T_\\lambda v, f_i\\big\\rangle=\\sum_{k=1}^n \\phi_k(v)\\cdot  \\big\\langle u_k, f_i\\big\\rangle =\\phi_k(v)\\cdot \\delta_{i,k}$  \n",
    "$\\implies \\phi_k(v)=0$ for $1\\leq k\\leq n\\implies v \\in \\ker T_\\lambda v \\implies v=0$   \n",
    "as $ T_\\lambda v =0\\implies v \\in \\text{span}\\big\\{x_1,\\dots, x_n\\big\\}$ and $\\sum_{k=1}^n \\phi_k(v)\\cdot u_k= \\sum_{k=1}^n 0\\cdot u_k=0$ and the map $v\\in\\text{span}\\big\\{x_1,\\dots, x_n\\big\\}\\mapsto \\sum_{k=1}^n \\phi_k(v)\\cdot u_k$ is invertible \n",
    "[e.g. the $u_k$ are linearly independent by checking $\\langle u_k, f_i\\rangle$ so this is a surjective linear map from an n-dimensional vector space to an $n-$dimensional vector space hence injective by rank-nullity]  \n",
    "conclude $\\dim \\ker B_\\lambda =0$  \n",
    "\n",
    "Now consider for arbitrary $x\\in X$   \n",
    "$\\big\\langle B_\\lambda x , f_p\\big\\rangle=\\big\\langle T_\\lambda x , f_p\\big\\rangle + \\sum_{k=1}^n \\phi_k(x)\\cdot \\big\\langle u_k , f_p\\big\\rangle=\\big\\langle  x , (T^*)_\\overline{\\lambda} f_p\\big\\rangle + \\sum_{k=1}^n \\phi_k(x)\\cdot \\big\\langle u_k , f_p\\big\\rangle=\\big\\langle  x , 0\\big\\rangle + \\sum_{k=1}^n \\phi_k(x)\\cdot \\delta_{k,p}=0$  \n",
    "i.e. $f_p$ kills $\\text{image }B_\\lambda\\iff f_p\\in \\left(\\text{image }B_\\lambda\\right)^\\perp=\\ker (T^*)_\\overline{\\lambda}$  \n",
    "where the iff is the definition on page 49, and the equality is Prop 5.2.8(i), thus  \n",
    "$\\dim \\ker (T^*)_\\overline{\\lambda}\\gt 0 = \\dim \\ker T_\\lambda$ \n",
    "which contradicts Prop 5.2.9 (Fredholm's first theorem)    \n",
    "\n",
    "**suppose for contradiction** that $n\\gt p$   \n",
    "(this is essentially the mirror image of the preceding argument)  \n",
    "$g \\in \\ker G_\\overline{\\lambda}\\implies -(T^*)_\\overline{ \\lambda}^*g = \\sum_{k=1}^p g(u_k)\\cdot \\phi_k$    \n",
    "$\\implies 0 =\\big\\langle  x_i, 0\\big\\rangle =\\big\\langle  x_i,  G_\\overline{\\lambda}g\\big\\rangle =\\big\\langle  x_i, (T^*)_\\overline{ \\lambda}^*g\\big\\rangle+ \\sum_{k=1}^p g(u_k)\\cdot\\big\\langle x_i, \\phi_k\\big\\rangle=\\big\\langle  T_\\lambda x_n, g\\big\\rangle+ \\sum_{k=1}^p g(u_k)\\cdot \\delta_{k,n}=0+\\sum_{k=1}^p g(u_k)\\cdot \\delta_{k,n}$  \n",
    "$\\implies  g(u_k)=0$ for $1\\leq k\\leq p\\implies g\\in \\ker (T^*)_\\overline{ \\lambda}^*\\implies g=0$  \n",
    "since $g\\in \\text{span }\\big\\{f_1,\\dots, f_p\\big\\}$ and $\\sum_{k=1}^p g(u_k)\\cdot \\phi_k = \\sum_{k=1}^p 0\\cdot \\phi_k =0$ but again the mapping  \n",
    "$g\\in \\text{span }\\big\\{f_1,\\dots, f_p\\big\\}\\mapsto \\sum_{k=1}^p g(u_k)\\cdot \\phi_k $ is a surjective linear map between $p$ dimensional vector spaces hence invertible (the $\\phi_i$ are linearly independent as can be confirmed by checking against $x_j$)\n",
    "$\\implies \\dim \\ker  G_\\overline{\\lambda}=0$  \n",
    "\n",
    "Now consider arbitrary $f \\in X^*$  \n",
    "$\\big\\langle x_n, (G^*)_\\overline {\\lambda} f\\big\\rangle=\\big\\langle x_n, (T^*)_\\overline {\\lambda} f\\big\\rangle+\\sum_{k=1}^p \\overline {g(u_k)}\\cdot\\big\\langle x_n,  \\phi_k\\big\\rangle=\\big\\langle x_n, (T^*)_\\overline {\\lambda} f\\big\\rangle +\\sum_{k=1}^p \\overline {g(u_k)}\\cdot 0=\\big\\langle T_\\lambda x_n, f\\big\\rangle=\\big\\langle 0, f\\big\\rangle=0$  \n",
    "i.e. $x_n$ kills $\\text{image }(G^*)_\\overline {\\lambda}\\iff x_n\\in\\big(\\text{image }(G^*)_\\overline{\\lambda}\\big)_\\perp=\\ker G_\\lambda$ per Prop 5.2.8(ii)  \n",
    "$\\implies \\dim \\ker G_\\lambda\\gt 0 =\\dim \\ker (G^*)_\\overline {\\lambda}$  \n",
    "which contradicts Prop 5.2.9  \n",
    "\n",
    "\n",
    "**conclude** $n= p$   "
   ]
  },
  {
   "cell_type": "code",
   "execution_count": null,
   "id": "b1c8ebbf",
   "metadata": {},
   "outputs": [],
   "source": []
  },
  {
   "cell_type": "code",
   "execution_count": null,
   "id": "22879d9e",
   "metadata": {},
   "outputs": [],
   "source": []
  }
 ],
 "metadata": {
  "kernelspec": {
   "display_name": "Python 3 (ipykernel)",
   "language": "python",
   "name": "python3"
  },
  "language_info": {
   "codemirror_mode": {
    "name": "ipython",
    "version": 3
   },
   "file_extension": ".py",
   "mimetype": "text/x-python",
   "name": "python",
   "nbconvert_exporter": "python",
   "pygments_lexer": "ipython3",
   "version": "3.8.16"
  }
 },
 "nbformat": 4,
 "nbformat_minor": 5
}
