{
 "cells": [
  {
   "cell_type": "markdown",
   "id": "f791defd",
   "metadata": {},
   "source": [
    "**7.18** Show that if $A,B\\in B(E)$ are invertible *iff* both $AB$ and $BA$ are invertible [where invertible is taken to mean has a bounded inverse]    \n",
    "The forward  directions is immediate  \n",
    "\n",
    "For the other direction consider e.g.  \n",
    "$A^{-1}:=(BA)^{-1}B$ which is bounded and since $AB$ is invertible we know $A$ is surjective  [since $A$ has a right inverse given by $B(BA)^{-1}$] hence any $v\\in V$ may be written as $Ax=v$ for some $x$ hence   \n",
    "\n",
    "$A^{-1}v=(BA)^{-1}Bv = (BA)^{-1}B(Ax) = x$  as required; put differently if $x \\in \\ker A\\implies 0 = Ax\\implies 0=(BA)^{-1}B0 =(BA)^{-1}B(Ax) = x$ hence $A$ is injective and the earlier stated right inverse $B(BA)^{-1}$ is a left inverse as well hence it is *the inverse* of $A$.  \n",
    "\n",
    "By nearly identical reasoning, setting $B^{-1}:= (AB)^{-1}A$ gives the result for $B$'s inverse, or just observe that $B=(BA)(A^{-1})$ the product of two invertible operators $\\implies B^{-1}=A(BA)^{-1}$ "
   ]
  },
  {
   "cell_type": "markdown",
   "id": "278bce42",
   "metadata": {},
   "source": [
    "**7.19**   \n",
    "Show that if $A,B \\in B(E)$ and $I-AB$ is invertible then $I-BA$ is also invertible with inverse $I+ B(I-AB)^{-1}A$ \n",
    "\n",
    "checking left multiplication by $I-BA$ [which shows commutativity]     \n",
    " $(I-BA)(I+ B(I-AB)^{-1}A)=(I+ B(I-AB)^{-1}A) - [BA + BAB(I-AB)^{-1}A]$  \n",
    " $ =(I+ B(I-AB)^{-1}A) - [BA + B(I-AB)^{-1}ABA]=(I+ B(I-AB)^{-1}A)(I-BA)$  \n",
    " where the key step is $AB$ and $(I-AB)$ commute so $AB$ commutes with $(I-AB)^{-1}$ [a basic group theoretic result]   \n",
    " \n",
    "checking right multiplication by $I-BA$   \n",
    " $(I+ B(I-AB)^{-1}A)(I-BA) =I-BA+ (B(I-AB)^{-1}A)(I-BA)=I-BA+ (B(I-AB)^{-1}(I-AB)A= I-BA+BA=I$  \n",
    " "
   ]
  },
  {
   "cell_type": "code",
   "execution_count": null,
   "id": "49ffe4e3",
   "metadata": {},
   "outputs": [],
   "source": []
  },
  {
   "cell_type": "markdown",
   "id": "e40c3372",
   "metadata": {},
   "source": [
    "**7.21**  \n",
    "Let $H,K$ be Hilbert spaces and  let $L\\in  B(H,K)$.  Show that $T^*T$ is Hermitian and $\\Vert T^*T\\Vert =\\Vert T \\Vert^2$  \n",
    "\n",
    "being self-adjoint is immediate and  \n",
    "$\\Vert T^* T\\Vert =\\sup_{\\Vert x \\Vert =1} \\langle T^* Tx,x\\rangle =\\sup_{\\Vert x \\Vert =1} \\langle  Tx,Tx\\rangle =\\sup_{\\Vert x \\Vert =1} \\Vert Tx\\Vert^2 = \\Vert T\\Vert^2 $  \n",
    "where the 1st equality is Property 6.1.5 from Eidelman et al \n",
    "\n",
    "$\\implies  \\Vert T\\Vert^2 = \\Vert T^* T\\Vert \\leq \\Vert T^*\\Vert \\cdot \\Vert T\\Vert $  \n",
    "$\\implies  \\Vert T\\Vert\\leq  \\Vert T^*\\Vert  $  \n",
    "\n",
    "and by re-running the argument with $A:=T^*$ we get  \n",
    "$\\implies  \\Vert A\\Vert^2 = \\Vert A^* A\\Vert \\leq \\Vert A^*\\Vert \\cdot \\Vert A\\Vert $  \n",
    "$\\implies \\Vert T^*\\Vert= \\Vert A\\Vert\\leq  \\Vert A^*\\Vert =\\Vert T\\Vert $  \n",
    "\n",
    "$\\implies  \\Vert T\\Vert= \\Vert T^*\\Vert  $  "
   ]
  },
  {
   "cell_type": "markdown",
   "id": "c27d506a",
   "metadata": {},
   "source": [
    "**7.29**  \n",
    "the 1st part of this, that $(\\text{image A})^\\perp = \\ker A^*$ and $\\overline{\\text{image A}}=\\big((\\text{image A})^\\perp\\big)^\\perp = (\\ker A^*)^\\perp$  is covered by ex 4.8.24 in Eidelman et al [as well as chapter 2 materials of that book]  \n",
    "\n",
    "for $A\\in B(H)$ show that $\\ker A^*A=\\ker A$  \n",
    "suppose $a \\in \\ker A$  \n",
    "$\\implies 0=\\langle Ax,Ax\\rangle =\\langle A^*Ax,x\\rangle\\implies x \\in \\ker A^*A$  \n",
    "where the implication comes from taking the square root i.e. $\\langle A^*Ax,x\\rangle=\\langle \\sqrt{A^*A}x,\\sqrt{A^*A}x\\rangle \\implies x \\in \\ker\\sqrt{A^*A}\\implies x \\in \\ker A^*A$  \n",
    "which is Corollary 6.3.6 in Eidelman et al  \n",
    "\n",
    "or by recognizing that $A^*A$ induces a semi-inner product given by $\\langle A^*A x,y\\rangle$ so e.g. using Gram matrices, select arbitrary $w \\in H$   \n",
    "\n",
    "$G:=\\displaystyle \\left[\\begin{matrix}\\langle A^*A x, x\\rangle & \\langle A^*A w, x\\rangle\\\\ \\langle A^*A x, w\\rangle & \\langle A^*A w, w\\rangle\\end{matrix}\\right]=\\displaystyle \\left[\\begin{matrix} 0 & \\langle A^*A w, x\\rangle\\\\ \\langle A^*A x, w\\rangle & \\langle A^*A w, w\\rangle\\end{matrix}\\right]$   \n",
    "\n",
    "For any $\\mathbf u\\in \\mathbb C^2$  \n",
    "$\\mathbf u^* G \\mathbf u=\\big\\langle A^*A (u_1\\cdot x + u_2\\cdot w), u_1\\cdot x+u_2\\cdot w\\big\\rangle\\geq 0$  \n",
    "$\\implies G\\succeq \\mathbf 0\\implies \\displaystyle \\left[\\begin{matrix} 0 & 0 \\\\ 0 & \\langle A^*A w, w\\rangle\\end{matrix}\\right]$  \n",
    "[check $\\det G\\geq 0$ or write $G=B^*B$]    \n",
    "$\\implies A^*A x\\in H^\\perp$ since $y$ was arbitrary $\\implies A^*A x = 0$   "
   ]
  },
  {
   "cell_type": "markdown",
   "id": "4c684e6f",
   "metadata": {},
   "source": [
    "**7.30**  \n",
    "let $A\\in B(H)$, then referencing the prior problem   \n",
    "$\\overline{\\text{image }A^*}= \\big(\\ker A\\big)^\\perp= \\big(\\ker A^*A\\big)^\\perp=\\overline{\\text{image }A^*A}$  \n"
   ]
  },
  {
   "cell_type": "markdown",
   "id": "a9cac422",
   "metadata": {},
   "source": [
    "**7.39**  \n",
    "Let $A,B \\in B(E)$, a Banach space.  Show that $\\sigma(AB)$ and $\\sigma(BA)$ are the same except possibly for point 0.  [note regarding $0$ consider the left and right shift operators on $\\mathscr l_2$ where $AB =\\text{id}$ but $(BA)^2=B(AB)A=BA$ is idempotent but not injective [since $A\\mathbf e_1=0$] hence not the identity so not invertible]  \n",
    "\n",
    "if $\\lambda \\in \\mathbb C\\sim\\big\\{0\\big\\}$  is a regular point of $AB$ then  \n",
    "\n",
    "$A':=\\lambda^{-1}A$  \n",
    "so $1$ is a regular point of $A'B$ i.e. $A'B-I$ is invertible hence $BA'-I$ is as well by problem 7.19.  Similarly if $\\lambda \\in \\mathbb C\\sim\\big\\{0\\big\\}$  is a regular point of $BA$ then $BA'-I$ is invertible hence $A'B-I$ is as well by problem 7.19 [with the symbols reversed].\n",
    "\n"
   ]
  },
  {
   "cell_type": "markdown",
   "id": "11344e71",
   "metadata": {},
   "source": [
    "**8.12**  \n",
    "Show that if $A^k= 0$ for some $k\\in \\mathbb N$ for $A\\succeq \\mathbf 0$ then $A= \\mathbf0$.  [$A$ being compact like in the problem statement isn't really needed though the author confines the sqrt of general positive bounded operator to an appendix and wants us to focus on the easier compact case]    \n",
    "\n",
    "let $k$ be the minimum natural number such that $A= \\mathbf 0$.  \n",
    "\n",
    "If $k=2m$ for $m\\in \\mathbb N$ then for arbitrary $x\\in H$ we have   \n",
    "$\\langle A^kx,x\\rangle =\\langle A^mx, A^mx\\rangle\\implies \\ker A^m =H\\implies A^m=0$, a contradiction  \n",
    "\n",
    "Now if $k\\% 2= 1$ we may instead consider $B:=\\sqrt A$ and $B^{2k}=0\\implies B^k=0$ per the preceding argument hence \n",
    "$\\implies \\mathbf 0=B^k = A^\\frac{k}{2}=A^\\frac{k}{2}B=A^\\frac{k+1}{2}$ where $\\frac{k+1}{2}\\geq k$ by assumption   \n",
    "$ \\implies k+1\\geq 2k\\implies k=1$  \n",
    "*alternatively if we wanted to avoid using the square-root* we could mimic the approach in ex 7.29 and consider the semi-inner product given by  $(x,y)\\mapsto\\langle A x, y\\rangle$ and consider for arbitrary $x,y\\in H$ that $\\langle A A^\\frac{k-1}{2}x,A^\\frac{k-1}{2}y\\rangle =0\\implies \\text{image }A^\\frac{k-1}{2}\\subseteq \\ker A $  since any $v\\in \\text{image }A^\\frac{k-1}{2}$ may be written as $v =A^\\frac{k-1}{2}x$  and consider arbitrary $y\\in H$ then  \n",
    "\n",
    "$G:=\\displaystyle \\left[\\begin{matrix}\\langle A v , v\\rangle & \\langle Av, y\\rangle\\\\ \\langle Ay, v\\rangle & \\langle A y, y\\rangle\\end{matrix}\\right]=\\displaystyle \\left[\\begin{matrix}0 & *\\\\ * & \\langle A y, y\\rangle\\end{matrix}\\right]$   \n",
    "where each $*=0$ by positive semi-definiteness of $G$ i.e. $\\langle Av, y\\rangle=0$ for arbitrary $y \\in H$, including $y:=Av$ hence $Av=0$.   Thus for arbitrary $x\\in H$  \n",
    "\n",
    "$AA^\\frac{k+1}{2} x =AA^\\frac{k-1}{2}x = 0\\implies AA^\\frac{k+1}{2}=0$  \n",
    "$\\implies \\frac{k+1}{2}\\geq k\\implies k+1\\geq 2k\\implies k=1$ \n",
    "\n"
   ]
  },
  {
   "cell_type": "markdown",
   "id": "7aa88a27",
   "metadata": {},
   "source": [
    "**8.13**  \n",
    "Let $A$ be a compact Hermitian operator on a Hilbert space $H$.  Show that if $A$ has infinite rank then the image of $A$ is not closed in $H$.  If $\\text{image} A = \\overline {\\text{image} A}$ then there is some $\\delta \\gt 0$ such that $\\Vert Ax \\Vert \\geq \\delta \\cdot \\Vert x\\Vert $ for all $x \\in (\\ker A)^\\perp=\\overline{\\text{image }A}$ per MacCluer ex 3.27.  \n",
    "\n",
    "Let the operator $T$ be the restriction of $A$ to $\\text{image A}$.  Note by checking the definition any bounded sequence $v_k \\in \\text{image }A$ we have $Tv_k=Av_k$ has a convergent [cauchy] subsequence hence $T$ is compact.  \n",
    "\n",
    "But we know that $T$ is invertible [ex 6.5.12 from Eidelman et al] which implies $TT^{-1}=I$ is compact hence $A$ must be finite dimensional.  Alternatively compare $\\Vert Tx \\Vert \\geq \\delta \\cdot \\Vert x\\Vert $ with the spectral theorem for compact self-adjoint operators [Theorem 8.15 in this text].   "
   ]
  },
  {
   "cell_type": "code",
   "execution_count": null,
   "id": "6edfed9a",
   "metadata": {},
   "outputs": [],
   "source": []
  },
  {
   "cell_type": "markdown",
   "id": "d99387ab",
   "metadata": {},
   "source": [
    "**8.15**  \n",
    "**pending**"
   ]
  },
  {
   "cell_type": "code",
   "execution_count": null,
   "id": "cb4f5323",
   "metadata": {},
   "outputs": [],
   "source": []
  },
  {
   "cell_type": "markdown",
   "id": "b41d7b30",
   "metadata": {},
   "source": [
    "**8.16 & 8.17 [combined]**  \n",
    "For compact $A$ write  \n",
    "$H = \\ker A^*A\\oplus \\overline{\\text{image }A^*A}$  \n",
    "a direct sum of orthogonal complements  \n",
    "\n",
    "I assume $A\\neq 0$ as the below results trivially hold for the zero operator.  \n",
    "\n",
    "For $y \\in \\ker A^*A$ define $Uy:=0$ and  \n",
    "\n",
    "for $z\\in\\overline{\\text{image }A^*A}$, as in problem 8.16, define $U$ as     \n",
    "$U\\big(\\sum_{n=1}^\\infty \\alpha_n\\cdot \\varphi_n\\big)  = \\sum_{n=1}^\\infty\\alpha_n\\cdot \\lambda_n^\\frac{-1}{2} \\cdot A \\varphi_n$ \n",
    "where all $\\lambda_n\\gt 0$ since $A^*A$ is injective on $\\overline{\\text{image }A^*A}=\\big(\\ker A^*A\\big)^\\perp$  \n",
    "[alternatively reference Eidelman et al Theorem 6.2.3]  \n",
    "\n",
    "noting the $\\varphi_n$ form an orthonormal basis for $\\overline{\\text{image }A^*A}$ so $z =\\sum_{k=1}^\\infty \\langle z,\\varphi_n\\rangle \\cdot \\varphi_n$ and set $\\alpha_n:=\\langle z,\\varphi_n\\rangle $   \n",
    "[projection formula-- in particular $w:=z-\\sum_{k=1}^\\infty \\langle z,\\varphi_n\\rangle \\cdot \\varphi_n$ then $w\\perp \\ker A^*A$ and $w\\perp \\text{span} \\big\\{\\varphi_j\\big\\}\\implies w \\perp\\overline {\\text{image }A^*A}\\implies w=0$]  \n",
    "\n",
    "Then for $x \\in H$ we have $x=y+z$  \n",
    "$Ax = Az = A\\big(\\sum_{n=1}^\\infty \\alpha_n\\cdot \\varphi_n\\big)= \\sum_{n=1}^\\infty \\alpha_n\\cdot A\\varphi_n  = \\sum_{n=1}^\\infty \\lambda_n^\\frac{1}{2}\\cdot\\alpha_n\\cdot\\lambda_n^\\frac{-1}{2} \\cdot A \\varphi_n$  \n",
    "$= U\\big(\\sum_{n=1}^\\infty \\alpha_n\\cdot \\lambda_n^\\frac{1}{2}\\cdot\\varphi_n\\big)  = U \\big(A^*A\\big)^\\frac{1}{2}\\big(\\sum_{n=1}^\\infty \\alpha_n\\cdot\\varphi_n\\big)=U \\big(A^*A\\big)^\\frac{1}{2}z = U \\big(A^*A\\big)^\\frac{1}{2}x $  \n",
    "where at the end we use $\\ker \\sqrt{A^*A}=\\ker A^*A$ which holds by problem 7.29.  \n",
    "\n",
    "Note that $U$ has norm 1 since  \n",
    "$\\big\\Vert Ux\\big\\Vert^2= \\langle Ux,Ux \\rangle=\\langle Uz,Uz \\rangle= \\langle  z,U^*Uz \\rangle=\\langle \\sum_{n=1}^\\infty \\alpha_n\\cdot \\varphi_n , \\sum_{n=1}^\\infty \\alpha_n \\big(\\lambda_n^\\frac{-1}{2}\\big)^2\\cdot A^*A \\varphi_n\\rangle=\\langle \\sum_{n=1}^\\infty \\alpha_n\\cdot \\varphi_n , \\sum_{n=1}^\\infty \\alpha_n \\varphi_n\\rangle=\\sum_{n=1}^\\infty \\vert \\alpha_n\\vert^2$  \n",
    "$= \\big\\Vert z\\big\\Vert^2\\leq \\big\\Vert y\\big\\Vert^2 +  \\big\\Vert z\\big\\Vert^2=\\big\\Vert x\\big\\Vert^2$  \n",
    "and set e.g. $x:= \\varphi_1$ to meet the upper bound with equality  \n",
    "\n",
    "\n",
    "Thus we have a polar decomposition for compact $A$ on some [not necessarily separable] Hilbert space $H$. Now define $B_r$ as a rank $r$ approximation of $\\sqrt{A^*A}$ i.e.  \n",
    "$B_r x = B_r z = B_r\\big(\\sum_{n=1}^\\infty \\alpha_n\\cdot \\varphi_n\\big)=\\sum_{n=1}^r \\alpha_n\\cdot\\lambda_n^\\frac{1}{2}\\cdot \\varphi_n$  \n",
    "where $B_r$ is compact since it has finite rank and is self-adjoint, by checking $\\langle B_r x, B_r x\\rangle \\geq 0$ for all $x$ in our [complex] Hilbert space.  Then  $\\sqrt {A^*A}- B_r$ has maximum eigenvalue $\\lambda_{r+1}^\\frac{1}{2}$ and since all eigenvalues are non-negative this means it is the max modulus eigenvalue of a compact self-adjoint operator hence $\\big\\Vert \\sqrt{A^*A } B_r \\big\\Vert =\\lambda_r^\\frac{1}{2}$ by Theorem 8.10 [in Eidelman et al this is Property 6.2.1]  \n",
    "\n",
    "$\\implies \\big\\Vert U B_r-A\\big\\Vert = \\big\\Vert U\\big(B_r- \\sqrt{A^*A}\\big)\\big\\Vert\\leq \\big\\Vert U\\big\\Vert \\cdot \\big\\Vert B_r- \\sqrt{A^*A}\\big\\Vert = 1\\cdot \\lambda_r^\\frac{1}{2} \\to 0$  \n",
    "\n",
    "Conclude: every compact operator on a Hilbert spaces is the [norm] limit of a sequence of finite rank operators.  [Note: this does not hold on general Banach spaces due to some work Enflo].  \n",
    "\n",
    "\n",
    "\n"
   ]
  },
  {
   "cell_type": "code",
   "execution_count": null,
   "id": "4619fedd",
   "metadata": {},
   "outputs": [],
   "source": []
  },
  {
   "cell_type": "markdown",
   "id": "8619eab9",
   "metadata": {},
   "source": [
    "- - - - \n",
    "Now define $U_r$ as a rank $r$ approximation of $U$, i.e. $U_ry=0$ for $y\\in \\ker A^*A$ and   \n",
    "$U_r\\big(\\sum_{n=1}^\\infty \\alpha_n\\cdot \\phi_n\\big)  = \\sum_{n=1}^r\\alpha_n\\cdot \\lambda_n^\\frac{-1}{2} \\cdot A \\phi_n$ \n",
    "\n",
    "thus for $\\Vert x\\Vert =1$, as before we have $x=y+z$  \n",
    "\n",
    "$\\big\\Vert (U_r \\sqrt{A^*A}-A)x\\big\\Vert = \\big\\Vert (U_r-U) \\sqrt{A^*A}x\\big\\Vert= \\big\\Vert (U_r-U) \\sqrt{A^*A}z\\big\\Vert = \\big\\Vert (U_r-U)\\sum_{n=1}^\\infty \\alpha_n\\cdot \\lambda_n^\\frac{1}{2}\\cdot\\phi_n\\big\\Vert= \\big\\Vert \\sum_{r+1}^\\infty \\alpha_n\\cdot A\\phi_n\\big\\Vert$  \n",
    "\n"
   ]
  },
  {
   "cell_type": "code",
   "execution_count": null,
   "id": "39ad3681",
   "metadata": {},
   "outputs": [],
   "source": []
  },
  {
   "cell_type": "code",
   "execution_count": null,
   "id": "4c1d9964",
   "metadata": {},
   "outputs": [],
   "source": []
  },
  {
   "cell_type": "code",
   "execution_count": null,
   "id": "7d6181c4",
   "metadata": {},
   "outputs": [],
   "source": []
  },
  {
   "cell_type": "code",
   "execution_count": null,
   "id": "37cd3984",
   "metadata": {},
   "outputs": [],
   "source": []
  }
 ],
 "metadata": {
  "kernelspec": {
   "display_name": "Python 3 (ipykernel)",
   "language": "python",
   "name": "python3"
  },
  "language_info": {
   "codemirror_mode": {
    "name": "ipython",
    "version": 3
   },
   "file_extension": ".py",
   "mimetype": "text/x-python",
   "name": "python",
   "nbconvert_exporter": "python",
   "pygments_lexer": "ipython3",
   "version": "3.8.16"
  }
 },
 "nbformat": 4,
 "nbformat_minor": 5
}
