{
 "cells": [
  {
   "cell_type": "markdown",
   "id": "84bcbc8e",
   "metadata": {},
   "source": [
    "**ex 0.4.1**   \n",
    "Prove Prop 0.1.6:  \n",
    "let $f \\in  B[a,b]$.  For any partition $P$ of $[a,b]$ \n",
    "$m\\cdot(b-a)\\leq L(f,P)\\leq U(f,P)\\leq M\\cdot (b-a)$  \n",
    "where $m= \\inf_{x \\in [a,b]}f(x)$ and $M=\\sup_{x\\in [a,b]} f(x)$  \n",
    "\n",
    "*remark:*  \n",
    "this comes down to observing the point-wise bound   \n",
    "$m\\cdot (x_i-x_{i-1}) \\leq m_i\\cdot (x_i-x_{i-1}) \\leq M_i\\cdot (x_i-x_{i-1}) \\leq M\\cdot (x_i-x_{i-1})$  \n",
    "then summing over the bound  \n",
    "\n",
    "$m\\cdot (b-a)=\\sum_{i=1}^n m\\cdot (x_i-x_{i-1})\\leq \\sum_{i=1}^n m_i\\cdot (x_i-x_{i-1}) = L(f,P)\\leq U(f,P)\\leq  \\sum_{i=1}^n M_i\\cdot (x_i-x_{i-1})\\leq \\sum_{i=1}^n M\\cdot (x_i-x_{i-1})=M\\cdot (b-a)$\n",
    "\n"
   ]
  },
  {
   "cell_type": "code",
   "execution_count": null,
   "id": "fc8efe3b",
   "metadata": {},
   "outputs": [],
   "source": []
  },
  {
   "cell_type": "markdown",
   "id": "c09bf1f7",
   "metadata": {},
   "source": [
    "**ex 0.4.2**  \n",
    "Let $f(x) = 1$ when $0\\leq x \\leq 2$ and $=2$ if $2\\lt x \\leq 3$  \n",
    "\n",
    "(a) Show $f\\in R\\big[0,3\\big]$  \n",
    "using Theorem 0.2.4    \n",
    "consider the partition $P_{\\delta}$ given by $\\Big\\{\\big[0, 2-\\delta\\big], \\big[2-\\delta , 2+\\delta\\big], \\big[2+\\delta, 3\\big]\\Big\\}$   \n",
    "$L\\big(f,P_\\delta\\big) = 1 \\cdot(2+\\delta) + 2\\cdot(1-\\delta) = 4-\\delta $   \n",
    "$U\\big(f,P_\\delta\\big) = 1 \\cdot(2-\\delta) + 2\\cdot(1+\\delta) = 4+\\delta $   \n",
    "\n",
    "$\\implies U\\big(f, P_\\delta\\big) -L\\big(f, P_\\delta\\big)\\leq 2 \\delta  \\lt \\epsilon$  \n",
    "for any $\\epsilon\\gt 0$ by setting e.g. $\\delta:= \\frac{\\epsilon}{3}$   \n",
    "\n",
    "(b) Compute $\\int_0^3 f(x)dx$ using the definition of the Riemann Integral  \n",
    "we claim $\\int_{a}^b f(x) dx=4$ since \n",
    "\n",
    "$4-\\delta= L\\big(f,P_\\delta\\big) \\leq \\sup_P L(f,P)=\\int_a^b f(x)dx =\\inf_P U(f,P)\\leq U\\big(f,P_\\delta\\big)=4+\\delta$  \n",
    "where equality holds by part (a) and Def 0.1.9 and Def 0.1.7;  this reads   \n",
    "$4-\\delta\\leq \\sup_P L(f,P) \\leq 4+\\delta$ and $4-\\delta\\leq \\inf_P U(f,P) \\leq 4+\\delta\\implies \\sup_P L(f,P) = 4=\\inf_P U(f,P) $  \n",
    "since $\\delta \\in \\big(0,1\\big)$ may be made arbitrarily small   \n",
    "\n",
    "**remark:**  \n",
    "I could have skipped Theorem 0.2.4 and part (a) and just written  \n",
    "$4-\\delta= L\\big(f,P_\\delta\\big) \\leq \\sup_P L(f,P)\\leq \\inf_P U(f,P)\\leq U\\big(f,P_\\delta\\big)=4+\\delta$   \n",
    "then used a squeeze (e.g. with $\\delta_k:= 2^{-k}$ and taken a limit) to infer \n",
    "$ L\\big(f,P_\\delta\\big)=4 =  U\\big(f,P_\\delta\\big)\\implies f\\in R\\big[0,3\\big]$  \n",
    "solving (a) and (b) at the same time  \n"
   ]
  },
  {
   "cell_type": "code",
   "execution_count": null,
   "id": "a5c717fc",
   "metadata": {},
   "outputs": [],
   "source": []
  },
  {
   "cell_type": "markdown",
   "id": "61151ab6",
   "metadata": {},
   "source": [
    "**ex 0.4.3**  \n",
    "Let $f,g \\in R[a,b]$ with $f(x)\\leq g(x)$ for all $x\\in[a,b]$.  Prove that  \n",
    "$\\int_a^b f(x)dx \\leq \\int_a^b g(x)dx$  \n",
    "suppose for contradiction $\\int_a^b f(x)dx - \\int_a^b g(x)dx = 2 \\epsilon \\gt 0$  \n",
    "\n",
    "Being both Riemann integrable means there are suitable partitions $P_f, P_g$ and a common refinement $P$ such that Theorem 0.2.4 is met for $\\epsilon$  \n",
    "in particular $-L(g,P)  \\lt\\epsilon - U(g,P) $  \n",
    "\n",
    "$\\implies 2 \\epsilon = \\int_a^b f(x)dx - \\int_a^b g(x)dx \\leq U(f,P) + \\big(- L(g,P)\\big)\\leq  U(f,P) +\\big(\\epsilon - U(g,P)\\big)$  \n",
    "$\\implies  U(g,P) + \\epsilon \\leq  U(f,P) \\leq U(g,P)$ \n",
    "note the RHS follows since $M_i^{(f)}\\leq M_i^{(g)}$ (and summing over the point-wise bound)   \n",
    "conclude $0\\lt \\epsilon \\leq 0$ which is a contradiction.  \n",
    "\n",
    "*remarks:*  \n",
    "(i) it is probably a bit better to show this directly instead of using a contradiction  \n",
    "(ii) this is Theorem 0.3.2 while Theorem 0.3.1 is done via ex 0.4.14 & ex 0.4.15.  Nelson seems to indicate on page 10 that only the first of these appears in the exercises though that isn't right  "
   ]
  },
  {
   "cell_type": "code",
   "execution_count": null,
   "id": "f171ba14",
   "metadata": {},
   "outputs": [],
   "source": []
  },
  {
   "cell_type": "markdown",
   "id": "8110d620",
   "metadata": {},
   "source": [
    "**ex 0.4.4**   \n",
    "Give an example of a function $f$ with $f\\not\\in R[0,1]$ but $f^2 \\in R[0,1]$  \n",
    "\n",
    "*remark:*  \n",
    "Notation is a bit problematic here.  It isn't clear whether $f^2$ means $f(x)\\cdot f(x)$ or $f^2 = f\\circ f$.  However in either case consider  \n",
    "\n",
    "$f(x) := 2\\chi_{\\mathbb Q}(x) -1$ where $\\chi_{\\mathbb Q}(x)$ denotes the Dirichlet function from page 2. Then $f\\big(\\mathbb R\\big)=1$ irrespective of $f^2$ referring to multiplication or composition.  "
   ]
  },
  {
   "cell_type": "code",
   "execution_count": null,
   "id": "e2a88a92",
   "metadata": {},
   "outputs": [],
   "source": []
  },
  {
   "cell_type": "markdown",
   "id": "85388ae8",
   "metadata": {},
   "source": [
    "**ex 0.4.6** \n",
    "let $\\{f_n\\}$ be a sequence of functions with $f_n \\in R[a,b]$ for each $n$.  Suppose the sequence $\\{f_n\\}$ converges uniformly to $f$ on $[a,b]$.  Show that $f\\in R[a,b]$  \n",
    "\n",
    "Applying Theorem 0.2.4, we need to show, for any $\\epsilon \\gt 0$ that $U(f,P)-L(f,P)\\lt \\epsilon$   \n",
    "\n",
    "$U(f,P)-L(f,P)= \\big \\vert U(f,P)-L(f,P)\\big \\vert = \\big \\vert \\big(U(f,P)- U(f_n,P)\\big) + \\big(U(f_n,P) -L(f_n,P)\\big) + \\big(L(f_n,P) -L(f,P)\\big)\\big \\vert$  \n",
    "$\\leq \\big \\vert U(f,P)- U(f_n,P)\\big \\vert  +\\big \\vert U(f_n,P) -L(f_n,P)\\big \\vert + \\big \\vert U(f_n,P) -L(f,P)\\big \\vert $  \n",
    "$\\lt \\frac{\\epsilon}{3}+\\frac{\\epsilon}{3}+\\frac{\\epsilon}{3}$  \n",
    "$=\\epsilon$  \n",
    "\n",
    "where $\\big \\vert f_n(x)-f(x)\\big \\vert \\lt \\frac{\\epsilon}{(b-a)\\cdot 3}$ for all $n\\geq N$  by uniform convergence. So fix some $n$ and  \n",
    "$\\big \\vert U(f_n,P) -L(f_n,P)\\big \\vert \\lt \\frac{\\epsilon}{3}$ by choosing a suitable partition $P$ since $f_n$ is Riemann integrable (Theorem 0.2.4) and  \n",
    "\n",
    "\n",
    "$\\big \\vert U(f,P)- U(f_n,P)\\big \\vert  = \\big \\vert \\sum_{i=1}^n (M_i-M_i^{(f_n)})\\cdot (x_i-x_{i-1})\\big \\vert\\leq  \\sum_{i=1}^n \\big \\vert M_i-M_i^{(f_n)}\\big \\vert \\cdot (x_i-x_{i-1})\\leq  \\frac{\\epsilon}{(b-a)\\cdot 3} \\cdot \\sum_{i=1}^n  (x_i-x_{i-1})=  \\frac{\\epsilon}{3}$  \n",
    "$\\big \\vert L(f,P)- L(f_n,P)\\big \\vert  = \\big \\vert \\sum_{i=1}^n (m_i-m_i^{(f_n)})\\cdot (x_i-x_{i-1})\\big \\vert\\leq  \\sum_{i=1}^n \\big \\vert m_i-m_i^{(f_n)}\\big \\vert \\cdot (x_i-x_{i-1})\\leq  \\frac{\\epsilon}{(b-a)\\cdot 3} \\cdot \\sum_{i=1}^n  (x_i-x_{i-1})=  \\frac{\\epsilon}{3}$  \n",
    "\n",
    "**technical commentary:**  \n",
    "the way to interpret e.g. $\\big \\vert M_2 - M_2^{(f_n)}\\big \\vert \\leq \\frac{\\epsilon}{(b-a)\\cdot 3}$ is that while \n",
    "the supremum may not exist in the set, it is the limit of a sequence of points in that set so  \n",
    "$M_2 = \\lim_{k\\to \\infty} f(x^{(k)})$ and $M_2^{(f_n)} = \\lim_{j\\to \\infty} f_n(x^{(k)})$\n",
    "\n",
    "so if $M_2 \\geq  M_2^{(f_n)}$ then  \n",
    "$M_2 -  M_2^{(f_n)} = \\big \\vert M_2 -  M_2^{(f_n)}\\big \\vert = \\lim_{k\\to \\infty}\\big \\vert f(x^{(k)}) - M_2^{(f_n)}\\big \\vert \\leq \\lim_{k\\to \\infty}\\big \\vert f(x^{(k)}) - f_n(x^{(k)})\\big \\vert \\leq \\frac{\\epsilon}{(b-a)\\cdot 3}$   \n",
    "where the first inequality holds by definition of the supremum and the second since $\\big \\vert f(x_k) - f_n(x_k)\\big \\vert \\lt \\frac{\\epsilon}{(b-a)\\cdot 3}$ for all $k$; the case of $M_2 \\leq  M_2^{(f_n)}$ follows similarly          \n",
    "\n",
    "and for avoidance of doubt, when dealing with bounding $\\big \\vert m_2 - m_2^{(f_n)}\\big \\vert$  \n",
    "consider if $m_2 \\geq  m_2^{(f_n)}$ then  \n",
    "$m_2 -  m_2^{(f_n)} = \\big \\vert m_2 -  m_2^{(f_n)}\\big \\vert = \\lim_{j\\to \\infty}\\big \\vert m_2 - f_n(x^{(j)})\\big \\vert \\leq \\lim_{j\\to \\infty}\\big \\vert f(x^{(j)}) - f_n(x^{(j)})\\big \\vert \\leq \\frac{\\epsilon}{(b-a)\\cdot 3}$   \n"
   ]
  },
  {
   "cell_type": "markdown",
   "id": "3afd89e0",
   "metadata": {},
   "source": [
    "**remark:**  \n",
    "$\\int_a^b f_n(x)dx\\to \\int_a^b f(x)dx$  \n",
    "write $g_n: [a,b]\\longrightarrow \\mathbb R$ given by $g_n(x):= f_n(x) -f(x)$  \n",
    "and for any $\\epsilon \\gt 0$, then for all $n$ large enough \n",
    "$\\vert g_n(x) \\vert \\lt \\epsilon \\iff -\\epsilon \\lt g_n(x)\\lt \\epsilon$  \n",
    "\n",
    "Applying Theorem 0.3.1 (exercises 14 and 15) we have   \n",
    "$-\\epsilon\\cdot (b-a)\\lt \\int_{a}^b g_n(x) dx = \\int_{a}^b f_n(x) dx - \\int_{a}^b f(x) dx\\lt \\epsilon\\cdot (b-a)$  \n",
    "where the upper and lower bounds are from Theorem 0.3.2 (ex 3, compare $g_n$ to the constant function $=\\epsilon$) with $\\int_{a}^b \\epsilon dx = \\epsilon\\cdot (b-a)$ since $\\epsilon \\cdot (b-a) \\leq L(f,P)\\leq U(f,P)\\leq \\epsilon \\cdot (b-a)$ for any partition $P$   \n",
    "$\\implies \\big \\vert \\int_{a}^b f_n(x) dx - \\int_{a}^b f(x) dx \\big \\vert \\lt \\epsilon$ for all $n$ large enough  "
   ]
  },
  {
   "cell_type": "code",
   "execution_count": null,
   "id": "6725a6bb",
   "metadata": {},
   "outputs": [],
   "source": []
  },
  {
   "cell_type": "markdown",
   "id": "e6c2bc17",
   "metadata": {},
   "source": [
    "**ex 0.4.8**  \n",
    "Prove or modify and  then prove: let $f\\in R[a,b]$ and $[c,d]\\subseteq [a,b]$.  Then  \n",
    "\n",
    "$\\int_c^d f(x)dx \\leq \\int_a^b f(x)dx$  \n",
    "\n",
    "**modification:** insert: $f(x)\\geq 0$ and the statement holds \n",
    "\n",
    "**proof:**  \n",
    "First apply Theorem 0.3.3 to confirm that $\\int_c^d f(x)dx $ exists.  Then using Theorem 0.3.4 (twice) write  \n",
    "$\\int_a^b f(x)dx = \\int_a^c f(x)dx+\\int_c^d f(x)dx + \\int_c^b f(x)dx$ \n",
    "$\\implies \\int_c^d f(x)dx = \\int_a^c 0\\cdot f(x)dx+\\int_c^d f(x)dx + \\int_d^b 0\\cdot f(x)dx \\leq \\int_a^c f(x)dx+\\int_c^d f(x)dx + \\int_d^b f(x)dx=\\int_a^b f(x)dx$  \n",
    "\n",
    "where we know e.g.  \n",
    "$0=\\int_a^c 0\\cdot f(x)dx \\leq \\int_a^c f(x)dx $  \n",
    "with the equality given by ex 0.4.15 (w/ $k=0$ or obvious) and the upper bound comes from ex 0.4.3 (Theorem 0.3.2)"
   ]
  },
  {
   "cell_type": "markdown",
   "id": "94fe0423",
   "metadata": {},
   "source": [
    "**ex 0.4.9**  \n",
    "Prove or give a counterexample: Suppose $f\\in R[a,b]$ and there exists $k\\gt 0$ such that $f(x)\\geq k$ for all $x \\in[a,b]$.  Then $\\frac{1}{f}\\in R[a,b]$.  \n",
    "\n",
    "The statement is true; using Theorem 0.3.1 (ex 15) it suffices to show the Riemann Integrability of $\\frac{1}{g}$ with $g(x):= \\frac{f(x)}{k}$ (equivalently WLOG $f(x) \\geq 1$).  \n",
    "\n",
    "Since $g\\in R[a,b]$ we apply Theorem 0.2.4: for any $\\epsilon  \\gt 0$ we have some partition $P$ such that  (using Def 0.1.5)  \n",
    "$\\sum_{i=1}^n (M_i-m_i)\\cdot (x_i - x_{i-1})= U(f,P)-L(f,P)\\lt \\epsilon$  \n",
    "$\\implies  \\sum_{i=1}^n \\big(\\frac{1}{m_i}-\\frac{1}{M_i}\\big)\\cdot (x_i - x_{i-1}) \\leq  \\sum_{i=1}^n (M_i-m_i)\\cdot (x_i - x_{i-1})\\lt \\epsilon$  \n",
    "\n",
    "since for $x\\geq y\\geq 1$ we have $xy\\cdot\\big(\\frac{1}{y}-\\frac{1}{x}\\big)= x - y\\leq xy\\cdot \\big(x-y\\big)$  which holds since $1\\leq xy$  \n",
    "\n",
    "$\\implies U(g,P)-L(f,p)= \\sum_{i=1}^n \\big(\\frac{1}{m_i}-\\frac{1}{M_i}\\big)\\cdot (x_i - x_{i-1}) \\lt\\epsilon$  \n",
    "i.e. with $J:\\mathbb R_{\\gt 0}\\rightarrow \\mathbb R_{\\gt 0}$ given by $J(x) =\\frac{1}{x}$ we observe that e.g. for $M_i$ we have $f(x)\\leq M_i$ for all $x\\in [x_{i-1},x_i]$ and $f\\big(x^{(k)}\\big)\\to M_i$ for some sequence.  Now $J\\big(f(x)\\big)\\geq \\frac{1}{M_i}$ for all $x\\in [x_{i-1},x]$ by algebraic properties of the (positive) inversion map and $g\\big(x^{(k)}\\big)=J\\Big(f\\big(x^{(k)}\\big)\\Big)\\to J\\big(M_i\\big)=\\frac{1}{M_i}$ by continuity of $J$.  I.e. $\\frac{1}{M_i}=m_i^{(g)}$ and by nearly identical reasoning $\\frac{1}{m_i}=M_i^{(g)}$.  \n",
    "\n",
    "*remark:*  \n",
    "The fact that $f$ is bounded away from zero is vital.  if it was not, then $\\frac{1}{f}$ would not be a bounded function hence per Def 0.1.9 $\\frac{1}{f}$ would not be Riemann integrable.  \n",
    "\n",
    "\n"
   ]
  },
  {
   "cell_type": "markdown",
   "id": "ab299c23",
   "metadata": {},
   "source": [
    "**ex 0.4.13**   \n",
    "Let $f,g\\in B[a,b]$. Show that for any partition $P$ of $[a,b]$  \n",
    "$L\\big(f,P\\big) +L\\big(g,P\\big) \\leq L\\big(f+g,P\\big)\\text{ and } U\\big(f +g,P\\big)\\leq U\\big(f,P\\big) + U\\big(g,p\\big)$   \n",
    "[*errata* note: the book had $L(f,P) +L(g,P)$ on RHS of second inequality which of course is wrong]  \n",
    "\n",
    "ala exercise 1 this amounts to coming up with a point-wise bound and summing over the bound, i.e. we need to prove  \n",
    "$m_i^{(f)}+m_i^{(g)}\\leq m_i^{(f+g)}$ and $M_i^{(f+g)} \\leq M_i^{(f)}+M_i^{(g)}$  \n",
    "\n",
    "The fact that two choice are better than one for the $\\inf$ is a standard result from intro to real analysis that we can prove via sequences. For some well chosen sequence $x^{(k)}$   \n",
    "\n",
    "$m_i^{(f+g)}= \\inf _{x\\in{x_{i-1},x_i}}\\Big(f(x)+g(x)\\Big) = \\lim_{k\\to \\infty}\\Big(f\\big(x^{(k)}\\big) + g\\big(x^{(k)}\\big)\\Big)\\geq \\inf _{x\\in{x_{i-1},x_i}}f(x)+\\inf _{x\\in{x_{i-1},x_i}}g(x)=m_i^{(f)}+m_i^{(g)} $  \n",
    "where by definition $f\\big(x^{(k)}\\big)\\geq \\inf _{x\\in{x_{i-1},x_i}}f(x)$ for all $k$ and $g\\big(x^{(k)}\\big)\\Big)\\geq \\inf _{x\\in{x_{i-1},x_i}}g(x)$ for all $k$ so the bounds hold in the limit as well  \n",
    "\n",
    "Similarly for some other well chosen sequence $x^{(k)}$   \n",
    "$M_i^{(f+g)}= \\sup _{x\\in{x_{i-1},x_i}}\\Big(f(x)+g(x)\\Big) = \\lim_{k\\to \\infty}\\Big(f\\big(x^{(k)}\\big) + g\\big(x^{(k)}\\big)\\Big)\\leq \\sup _{x\\in{x_{i-1},x_i}}f(x)+\\sup _{x\\in{x_{i-1},x_i}}g(x)=m_i^{(f)}+m_i^{(g)} $  \n",
    "\n"
   ]
  },
  {
   "cell_type": "markdown",
   "id": "b1c57640",
   "metadata": {},
   "source": [
    "**ex 0.4.14**   \n",
    "Prove part (i.) of Theorem 0.3.1, that if $f, g \\in R[a,b]$ then  \n",
    "$\\int_{a}^b (f+g)(x) dx = \\int_{a}^b f(x) dx + \\int_{a}^b g(x) dx$    \n",
    "\n",
    "We can prove both Riemann Integrability of $(f+g)$ and the calculation via setting up a squeeze.  The prior exercise combined with the setup for Def 0.1.7 tells us for any Partition $P$     \n",
    "$L\\big(f,P\\big) +L\\big(g,P\\big) \\leq L\\big(f+g,P\\big)\\leq U\\big(f +g,P\\big)\\leq U\\big(f,P\\big) + U\\big(g,P\\big)$    \n",
    "\n",
    "using sequences we have  \n",
    "$\\sup L\\big(f,P\\big)=\\lim_{k\\to \\infty}  L\\big(f,P_{k^{(f)}}\\big) $  \n",
    "$\\sup L\\big(g,P\\big)=\\lim_{k\\to \\infty}  L\\big(f,P_{k^{(g)}}\\big)  $ \n",
    "and let $P_k^*$ be a common refinement for each $k$.  Application of Lemma $0.2.2$ and taking limits yields  a squeeze \n",
    "$\\sup L\\big(f,P\\big)=\\lim_{k\\to \\infty}  L\\big(f,P_{k^{(f)}}\\big) \\leq \\lim_{k\\to \\infty}  L\\big(f,P_{k}^*\\big) \\leq \\sup L\\big(f,P\\big)\\text{ & }$$\\sup L\\big(g,P\\big)=\\lim_{k\\to \\infty}  L\\big(g,P_{k^{(g)}}\\big) \\leq \\lim_{k\\to \\infty}  L\\big(g,P_{k}^*\\big) \\leq \\sup L\\big(g,P\\big)$  \n",
    "**notice this holds with any further common refinement involving** $P_k^*$ (and of course a common refinement involving that common refinement and so on)   \n",
    "\n",
    "By almost identical reasoning we can write $U\\big(f,P\\big) + U\\big(g,p\\big)$ as a limit of a sequence by taking  common refinement of two sequences, yielding  \n",
    "$\\inf U\\big(f,P\\big)= \\lim_{j\\to -\\infty}  U\\big(f,P_{j}^*\\big) \\text{ & }$$\\inf U\\big(g,P\\big)= \\lim_{j\\to -\\infty}  U\\big(g,P_{j}^*\\big) $  \n",
    "\n",
    "Finally, consider $P_k^{**}$ the common refinement of $P_k^*$ and $P_{-k}^*$ giving    \n",
    "$L\\big(f,P_k^{**}\\big) +L\\big(g,P_k^{**}\\big) \\leq L\\big(f+g,P_k^{**}\\big)\\leq U\\big(f +g,P_k^{**}\\big)\\leq U\\big(f,P_k^{**}\\big) + U\\big(g,P_k^{**}\\big)$    \n",
    "taking limits and applying Def 0.1.7 and Def 0.1.9 we get    \n",
    "$\\int_{a}^b f(x) dx + \\int_{a}^b g(x) dx \\leq \\lim_{k\\to \\infty}L\\big(f+g,P_k^{**}\\big)\\leq \\lim_{k\\to \\infty} U\\big(f +g,P_k^{**}\\big)\\leq \\int_{a}^b f(x) dx + \\int_{a}^b g(x) dx$  \n",
    "$\\implies$  Theorem 0.2.4 is met by choosing $P_k^{**}$ with large enough $k$, so $\\int_{a}^b (f+g)(x) dx$ exists and $\\int_{a}^b (f+g)(x) dx=\\int_{a}^b f(x) dx + \\int_{a}^b g(x) dx$   \n",
    "\n",
    "For avoidance of doubt regarding the calculation:   \n",
    "consider $\\lim_{k\\to \\infty} U(f+g, P^{(k)})=\\inf_P  U(f+g, P)$ and the common refinement $P^{***}_k$ of $P^{(k)}$ and $P_k^{**}$, we still have   \n",
    "$\\inf_P  U(f+g, P)\\leq \\lim_{k\\to \\infty}  U(f+g, P_k^{**})\\leq \\lim_{k\\to \\infty} U(f+g, P^{(k)})=\\inf_P  U(f+g, P)\\text{  and  }$  \n",
    "$L\\big(f,P_k^{***}\\big) +L\\big(g,P_k^{***}\\big) \\leq L\\big(f+g,P_k^{***}\\big)\\leq U\\big(f +g,P_k^{***}\\big)\\leq U\\big(f,P_k^{***}\\big) + U\\big(g,P_k^{***}\\big)$    \n",
    "where taking limits yields yet another squeeze  \n"
   ]
  },
  {
   "cell_type": "markdown",
   "id": "04476132",
   "metadata": {},
   "source": [
    "**ex 0.4.15**   \n",
    "Prove part (ii.) of Theorem 0.3.1  \n",
    "for some sequence (as with the prior exercise we may first need two sequences then a common refinement)  \n",
    "\n",
    "$\\int_{a}^b f(x) dx = \\lim_{j\\to \\infty}L\\big(f,P_j\\big)= \\lim_{j\\to \\infty} U\\big(f,P_j\\big)$  \n",
    "\n",
    "**(a)** For $k\\geq 0$  \n",
    "$k\\cdot \\int_{a}^b f(x) dx = k\\cdot \\lim_{j\\to \\infty}L\\big(f,P_j\\big)=  \\lim_{j\\to \\infty} L\\big(k\\cdot f,P_j\\big) \\leq \\lim_{j\\to \\infty}U\\big(k\\cdot  f,P_j\\big) =k\\cdot \\lim_{j\\to \\infty} U\\big(f,P_j\\big)=k\\cdot \\int_{a}^b f(x) dx$  \n",
    "since multiplication is continuous and multiplication by non-negative numbers preserves (non-strict) ordering, so $k\\cdot f$ is Riemann Integrable per Theorem 0.2.4 and Lemma 0.2.2(ii) tells us $L\\big(k\\cdot f,P_j\\big)\\leq U\\big(k\\cdot f,P\\big)$ for any choice of $P$, so  \n",
    "$k\\cdot \\int_{a}^b f(x) dx =  \\lim_{j\\to \\infty}L\\big(k\\cdot f,P_j\\big)\\leq \\inf_{P} U\\big(k\\cdot f,P\\big) \\text{  &  }\\inf_{P} U\\big(k\\cdot f,P_j\\big) \\leq  k\\cdot \\int_{a}^b f(x) dx$  since $U\\big(k\\cdot  f,P_j\\big) \\to k\\cdot \\int_{a}^b f(x) dx$ so anything strictly larger cannot be an $\\inf$  \n",
    "\n",
    "**(b)** for $k=-1$   \n",
    "($k\\lt 0$ then follows by considering two steps -- first multiplying by suitable positive number, then re-scaling by $-1$)  \n",
    "\n",
    "This time the ordering is reversed, i.e. we have $U(f,P)\\mapsto L(-f,P)$ and $L(f,P)\\mapsto U(-f,P)$  \n",
    "$\\big[$e.g. consider the sequence form of $m_i^{(f)}= \\inf _{x\\in{x_{i-1},x_i}}f(x) \\leq f\\big(x^{(k)}\\big)$ where the ineguality is met with equality in the limit for well chosen $x^{(k)}$ but is valid as an inequality for all sequences.  Negating $f$ yields  $-m_i^{(f)}= -\\inf_{x\\in{x_{i-1},x_i}}f(x) \\geq -f\\big(x^{(k)}\\big)$ again being met with equality in the limit for well chosen $x^{(k)}$ but a valid inequality for all sequences so $-m_i^{(f)}= M_i^{(-f)}= \\sup_{x\\in{x_{i-1},x_i}}-f(x)\\big]$.  \n",
    "\n",
    "Theorem 0.2.4 applies to $f$ for any $\\epsilon \\gt 0$ yielding satisfactory $P$ so  \n",
    "$\\big \\vert L(-1\\cdot f,P)- U(-1\\cdot f,P)\\big\\vert = \\big \\vert -1\\cdot U(f,P)-(-1)\\cdot L(f,P)\\big\\vert = \\big \\vert U(f,P)-L(f,P)\\big\\vert \\lt \\epsilon$  \n",
    "hence $-f$ is Riemann Integrable.  And apply the prior exercise (i.e. part (i.) of Theorem 0.3.1) \n",
    "\n",
    "$0=\\int_{a}^b \\big(0\\cdot f(x)\\big)dx= \\int_{a}^b \\big(f(x) + -1\\cdot f(x)\\big)dx= \\int_{a}^b f(x)dx+\\int_{a}^b-1 \\cdot f(x)dx  \\implies  -\\int_{a}^b f(x)dx =\\int_{a}^b-1 \\cdot f(x)dx $  \n",
    "where the first equality is implied by part (a) of this exercise ($k=0$) or just taken as obvious from Def 0.1.7.  "
   ]
  },
  {
   "cell_type": "code",
   "execution_count": null,
   "id": "ce2e1cee",
   "metadata": {},
   "outputs": [],
   "source": []
  }
 ],
 "metadata": {
  "kernelspec": {
   "display_name": "Python 3 (ipykernel)",
   "language": "python",
   "name": "python3"
  },
  "language_info": {
   "codemirror_mode": {
    "name": "ipython",
    "version": 3
   },
   "file_extension": ".py",
   "mimetype": "text/x-python",
   "name": "python",
   "nbconvert_exporter": "python",
   "pygments_lexer": "ipython3",
   "version": "3.8.16"
  }
 },
 "nbformat": 4,
 "nbformat_minor": 5
}
